Formalize alternating directed paths and graphs based on adjacency Map

BFS/BFS.thy
@@ -1,10 +1,10 @@
 theory BFS
-  imports
+imports
     "../Map_Specs_Tbd"
     "../Misc_Tbd"
     "../Queue_Specs"
     "../Tbd"
-    "../Tbd_Graph_Tbd"
+    "../Tbd_Graph"
 begin
 
 record ('q, 'm) state =
@@ -12,215 +12,234 @@ record ('q, 'm) state =
   parent :: "'m"
 
 locale bfs =
-  G: finite_digraph where insert = insert +
-  Map where empty = Map_empty and update = update and delete = Map_delete and invar = Map_invar +
-  Queue where empty = Queue_empty and snoc = snoc and invar = Queue_invar
+  G: adjacency where Map_update = Map_update +
+  P: Map where
+  empty = P_empty and
+  update = P_update and
+  delete = P_delete and
+  lookup = P_lookup and
+  invar = P_invar +
+  Q: Queue where
+  empty = Q_empty and
+  is_empty = Q_is_empty and
+  snoc = Q_snoc and
+  head = Q_head and
+  tail = Q_tail and
+  invar = Q_invar and
+  list = Q_list
   for
-    insert :: "'a::linorder \<Rightarrow> 's \<Rightarrow> 's" and
-    Map_empty and
-    update :: "'a \<Rightarrow> 'a \<Rightarrow> 'm \<Rightarrow> 'm" and
-    Map_delete and
-    Map_invar and
-    Queue_empty and
-    snoc :: "'q \<Rightarrow> 'a \<Rightarrow> 'q" and
-    Queue_invar +
-  fixes src :: 'a
-  assumes src_mem_vertices: "src \<in> vertices"
+    Map_update :: "'a::linorder \<Rightarrow> 's \<Rightarrow> 'n \<Rightarrow> 'n" and
+    P_empty and
+    P_update :: "'a \<Rightarrow> 'a \<Rightarrow> 'm \<Rightarrow> 'm" and
+    P_delete and
+    P_lookup and
+    P_invar and
+    Q_empty and
+    Q_is_empty and
+    Q_snoc :: "'q \<Rightarrow> 'a \<Rightarrow> 'q" and
+    Q_head and
+    Q_tail and
+    Q_invar and
+    Q_list
+begin
 
-abbreviation (in bfs) dist :: "'a \<Rightarrow> enat" where
-  "dist \<equiv> Shortest_Dpath.dist edges src"
+abbreviation dist :: "'n \<Rightarrow> 'a \<Rightarrow> 'a \<Rightarrow> enat" where
+  "dist G \<equiv> Shortest_Dpath.dist (G.E G)"
 
-section \<open>BFS Algorithm\<close>
+abbreviation is_shortest_dpath :: "'n \<Rightarrow> 'a list \<Rightarrow> 'a \<Rightarrow> 'a \<Rightarrow> bool" where
+  "is_shortest_dpath G p u v \<equiv> dpath_bet (G.E G) p u v \<and> dpath_length p = dist G u v"
 
-definition (in bfs) init :: "('q, 'm) state" where
-  "init \<equiv>
-   \<lparr>queue = snoc Queue_empty src,
-    parent = Map_empty\<rparr>"
+section \<open>BFS algorithm\<close>
 
-definition (in bfs) cond :: "('q, 'm) state \<Rightarrow> bool" where
-  "cond s \<longleftrightarrow> \<not> is_empty (queue s)"
+definition init :: "'a \<Rightarrow> ('q, 'm) state" where
+  "init src \<equiv>
+   \<lparr>queue = Q_snoc Q_empty src,
+    parent = P_empty\<rparr>"
 
-definition (in bfs) discovered :: "('q, 'm) state \<Rightarrow> 'a \<Rightarrow> bool" where
-  "discovered s v \<longleftrightarrow> v = src \<or> v \<in> dom (parent s)"
+definition cond :: "('q, 'm) state \<Rightarrow> bool" where
+  "cond s \<longleftrightarrow> \<not> Q_is_empty (queue s)"
 
-definition (in bfs) discover :: "'a \<Rightarrow> 'a \<Rightarrow> ('q, 'm) state \<Rightarrow> ('q, 'm) state" where
+definition discovered :: "'a \<Rightarrow> ('q, 'm) state \<Rightarrow> 'a \<Rightarrow> bool" where
+  "discovered src s v \<longleftrightarrow> v = src \<or> P_lookup (parent s) v \<noteq> None"
+
+definition discover :: "'a \<Rightarrow> 'a \<Rightarrow> ('q, 'm) state \<Rightarrow> ('q, 'm) state" where
   "discover u v s \<equiv>
-   \<lparr>queue = snoc (queue s) v,
-    parent = update v u (parent s)\<rparr>"
+   \<lparr>queue = Q_snoc (queue s) v,
+    parent = P_update v u (parent s)\<rparr>"
 
-definition (in bfs) traverse_edge :: "'a \<Rightarrow> 'a \<Rightarrow> ('q, 'm) state \<Rightarrow> ('q, 'm) state" where
-  "traverse_edge u v s \<equiv>
-   if \<not> discovered s v then discover u v s
+definition traverse_edge :: "'a \<Rightarrow> 'a \<Rightarrow> 'a \<Rightarrow> ('q, 'm) state \<Rightarrow> ('q, 'm) state" where
+  "traverse_edge src u v s \<equiv>
+   if \<not> discovered src s v then discover u v s
    else s"
 
-function (in bfs) (domintros) loop :: "('q, 'm) state \<Rightarrow> ('q, 'm) state" where
-  "loop s =
+function (domintros) loop :: "'n \<Rightarrow> 'a \<Rightarrow> ('q, 'm) state \<Rightarrow> ('q, 'm) state" where
+  "loop G src s =
    (if cond s
     then let
-          u = head (queue s);
-          q = tail (queue s)
-         in loop (fold (traverse_edge u) (inorder (out_neighborhood u)) (s\<lparr>queue := q\<rparr>))
+          u = Q_head (queue s);
+          q = Q_tail (queue s)
+         in loop G src (fold (traverse_edge src u) (G.out_neighborhood G u) (s\<lparr>queue := q\<rparr>))
     else s)"
   by pat_completeness simp
 
-abbreviation (in bfs) bfs :: "('q, 'm) state" where
-  "bfs \<equiv> loop init"
+abbreviation bfs :: "'n \<Rightarrow> 'a \<Rightarrow> ('q, 'm) state" where
+  "bfs G src \<equiv> loop G src (init src)"
 
 section \<open>\<close>
 
-abbreviation (in bfs) fold :: "('q, 'm) state \<Rightarrow> ('q, 'm) state" where
-  "fold s \<equiv>
+abbreviation fold :: "'n \<Rightarrow> 'a \<Rightarrow> ('q, 'm) state \<Rightarrow> ('q, 'm) state" where
+  "fold G src s \<equiv>
    List.fold
-    (traverse_edge (head (queue s)))
-    (inorder (out_neighborhood (head (queue s))))
-    (s\<lparr>queue := tail (queue s)\<rparr>)"
+    (traverse_edge src (Q_head (queue s)))
+    (G.out_neighborhood G (Q_head (queue s)))
+    (s\<lparr>queue := Q_tail (queue s)\<rparr>)"
 
-abbreviation (in bfs) T :: "('q, 'm) state \<Rightarrow> 'a dgraph" where
-  "T s \<equiv> {(u, v) |u v. lookup (parent s) v = Some u}"
+abbreviation T :: "('q, 'm) state \<Rightarrow> 'a dgraph" where
+  "T s \<equiv> {(u, v) |u v. P_lookup (parent s) v = Some u}"
 
 section \<open>Convenience Lemmas\<close>
 
-subsection \<open>Queue_invar \<circ> queue\<close>
+subsection \<open>@{term "Q_invar \<circ> queue"}\<close>
 
-lemma (in bfs) invar_tail:
-  assumes "Queue_invar (queue s)"
+lemma tail_invar:
+  assumes "Q_invar (queue s)"
   assumes "cond s"
-  shows "Queue_invar (queue (s\<lparr>queue := tail (queue s)\<rparr>))"
-  using assms invar_tail
-  by (simp add: cond_def is_empty)
+  shows "Q_invar (queue (s\<lparr>queue := Q_tail (queue s)\<rparr>))"
+  using assms Q.invar_tail
+  by (simp add: cond_def Q.is_empty)
 
-subsection \<open>list \<circ> queue\<close>
+subsection \<open>@{term "Q_list \<circ> queue"}\<close>
 
-lemma (in bfs) list_queue_non_empty:
-  assumes "Queue_invar (queue s)"
+lemma list_queue_non_empty:
+  assumes "Q_invar (queue s)"
   assumes "cond s"
-  shows "list (queue s) \<noteq> []"
+  shows "Q_list (queue s) \<noteq> []"
   using assms
-  by (simp add: cond_def is_empty)
+  by (simp add: cond_def Q.is_empty)
 
-subsection \<open>invar \<circ> out_neighborhood\<close>
+subsection \<open>@{term "Q_head \<circ> queue"}\<close>
 
-lemma (in bfs) invar_out_neighborhood_if:
-  assumes "Queue_invar (queue s)"
-  assumes "set (list (queue s)) \<subseteq> vertices"
+lemma head_queue_mem_V:
+  assumes "Q_invar (queue s)"
+  assumes "set (Q_list (queue s)) \<subseteq> G.V G"
   assumes "cond s"
-  shows "G.invar (out_neighborhood (head (queue s)))"
+  shows "Q_head (queue s) \<in> G.V G"
   using assms list_queue_non_empty
-  by (fastforce simp add: list_head intro: G.invar_out_neighborhood)
+  by (auto simp add: Q.list_head)
 
 section \<open>Basic Lemmas\<close>
 
-subsection \<open>@{term bfs.discover}\<close>
+subsection \<open>@{term discover}\<close>
 
-subsubsection \<open>queue\<close>
+subsubsection \<open>@{term queue}\<close>
 
-lemma (in bfs) queue_discover_cong [simp]:
-  shows "queue (discover u v s) = snoc (queue s) v"
+lemma queue_discover_cong [simp]:
+  shows "queue (discover u v s) = Q_snoc (queue s) v"
   by (simp add: discover_def)
 
-subsubsection \<open>parent\<close>
+subsubsection \<open>@{term parent}\<close>
 
-lemma (in bfs) parent_discover_cong [simp]:
-  shows "parent (discover u v s) = update v u (parent s)"
+lemma parent_discover_cong [simp]:
+  shows "parent (discover u v s) = P_update v u (parent s)"
   by (simp add: discover_def)
 
-subsection \<open>@{term bfs.traverse_edge}\<close>
+subsection \<open>@{term traverse_edge}\<close>
 
-subsubsection \<open>queue\<close>
+subsubsection \<open>@{term queue}\<close>
 
-lemma (in bfs) queue_traverse_edge_cong:
-  shows "queue (traverse_edge u v s) = (if \<not> discovered s v then snoc (queue s) v else queue s)"
+lemma queue_traverse_edge_cong:
+  shows "queue (traverse_edge src u v s) = (if \<not> discovered src s v then Q_snoc (queue s) v else queue s)"
   by (simp add: traverse_edge_def)
 
-subsubsection \<open>Queue_invar \<circ> queue\<close>
+subsubsection \<open>@{term "Q_invar \<circ> queue"}\<close>
 
-lemma (in bfs) invar_queue_traverse_edge:
-  assumes "Queue_invar (queue s)"
-  shows "Queue_invar (queue (traverse_edge u v s))"
-  using assms invar_snoc
+lemma queue_traverse_edge_invar:
+  assumes "Q_invar (queue s)"
+  shows "Q_invar (queue (traverse_edge src u v s))"
+  using assms Q.invar_snoc
   by (simp add: queue_traverse_edge_cong)
 
-subsubsection \<open>list \<circ> queue\<close>
+subsubsection \<open>@{term "Q_list \<circ> queue"}\<close>
 
-lemma (in bfs) list_queue_traverse_edge_cong:
-  assumes "Queue_invar (queue s)"
+lemma list_queue_traverse_edge_cong:
+  assumes "Q_invar (queue s)"
   shows
-    "list (queue (traverse_edge u v s)) =
-     list (queue s) @ (if \<not> discovered s v then [v] else [])"
+    "Q_list (queue (traverse_edge src u v s)) =
+     Q_list (queue s) @ (if \<not> discovered src s v then [v] else [])"
   using assms
-  by (simp add: queue_traverse_edge_cong list_snoc)
+  by (simp add: queue_traverse_edge_cong Q.list_snoc)
 
-subsubsection \<open>lookup \<circ> parent\<close>
+subsubsection \<open>@{term "P_lookup \<circ> parent"}\<close>
 
-lemma (in bfs) lookup_parent_traverse_edge_cong:
-  assumes "Map_invar (parent s)"
+lemma lookup_parent_traverse_edge_cong:
+  assumes "P_invar (parent s)"
   shows
-    "lookup (parent (traverse_edge u v s)) =
+    "P_lookup (parent (traverse_edge src u v s)) =
      override_on
-      (lookup (parent s))
+      (P_lookup (parent s))
       (\<lambda>_. Some u)
-      (if \<not> discovered s v then {v} else {})"
+      (if \<not> discovered src s v then {v} else {})"
   using assms
-  by (simp add: traverse_edge_def map_update override_on_insert')
+  by (simp add: traverse_edge_def P.map_update override_on_insert')
 
-subsubsection \<open>Map_invar \<circ> parent\<close>
+subsubsection \<open>@{term "P_invar \<circ> parent"}\<close>
 
-lemma (in bfs) invar_parent_traverse_edge:
-  assumes "Map_invar (parent s)"
-  shows "Map_invar (parent (traverse_edge u v s))"
-  using assms invar_update
+lemma parent_traverse_edge_invar:
+  assumes "P_invar (parent s)"
+  shows "P_invar (parent (traverse_edge src u v s))"
+  using assms P.invar_update
   by (simp add: traverse_edge_def)
 
-subsubsection \<open>@{term bfs.T}\<close>
+subsubsection \<open>@{term T}\<close>
 
-lemma (in bfs) T_traverse_edge_cong:
-  assumes "Map_invar (parent s)"
-  shows "T (traverse_edge u v s) = T s \<union> (if \<not> discovered s v then {(u, v)} else {})"
+lemma T_traverse_edge_cong:
+  assumes "P_invar (parent s)"
+  shows "T (traverse_edge src u v s) = T s \<union> (if \<not> discovered src s v then {(u, v)} else {})"
   using assms
-  by (auto simp add: lookup_parent_traverse_edge_cong override_on_def discovered_def dom_def)
+  by (auto simp add: lookup_parent_traverse_edge_cong override_on_def discovered_def)
 
-subsection \<open>@{term bfs.fold}\<close>
+subsection \<open>@{term fold}\<close>
 
-subsubsection \<open>Queue_invar \<circ> queue\<close>
+subsubsection \<open>@{term "Q_invar \<circ> queue"}\<close>
 
-lemma (in bfs) invar_queue_fold:
-  assumes "Queue_invar (queue s)"
+lemma queue_fold_invar:
+  assumes "Q_invar (queue s)"
   assumes "distinct l"
-  shows "Queue_invar (queue (List.fold (traverse_edge u) l s))"
+  shows "Q_invar (queue (List.fold (traverse_edge src u) l s))"
   using assms
-  by (induct l arbitrary: s) (simp_all add: invar_queue_traverse_edge)
+  by (induct l arbitrary: s) (simp_all add: queue_traverse_edge_invar)
 
-lemma (in bfs) invar_queue_fold_2:
-  assumes "G.invar (out_neighborhood (head (queue s)))"
-  assumes "Queue_invar (queue s)"
+lemma queue_fold_invar_2:
+  assumes "G.invar G"
+  assumes "Q_invar (queue s)"
   assumes "cond s"
-  shows "Queue_invar (queue (fold s))"
+  shows "Q_invar (queue (fold G src s))"
   using assms
-  by (auto intro: invar_tail G.inorder_distinct invar_queue_fold)
+  by (auto intro: G.out_neighborhood_distinct tail_invar queue_fold_invar)
 
-subsubsection \<open>list \<circ> queue\<close>
+subsubsection \<open>@{term "Q_list \<circ> queue"}\<close>
 
-lemma (in bfs) list_queue_fold_cong_aux:
-  assumes "Map_invar (parent s)"
+lemma list_queue_fold_cong_aux:
+  assumes "P_invar (parent s)"
   assumes "distinct (v # vs)"
-  shows "filter (Not \<circ> discovered (traverse_edge u v s)) vs = filter (Not \<circ> discovered s) vs"
+  shows "filter (Not \<circ> discovered src (traverse_edge src u v s)) vs = filter (Not \<circ> discovered src s) vs"
 proof (rule filter_cong)
   fix w
   assume "w \<in> set vs"
-  hence "discovered (traverse_edge u v s) w = discovered s w"
+  hence "discovered src (traverse_edge src u v s) w = discovered src s w"
     using assms
-    by (auto simp add: discovered_def dom_def lookup_parent_traverse_edge_cong override_on_insert')
-  thus "(Not \<circ> discovered (traverse_edge u v s)) w = (Not \<circ> discovered s) w"
+    by (auto simp add: discovered_def lookup_parent_traverse_edge_cong override_on_insert')
+  thus "(Not \<circ> discovered src (traverse_edge src u v s)) w = (Not \<circ> discovered src s) w"
     by simp
 qed simp
 
-lemma (in bfs) list_queue_fold_cong:
-  assumes "Queue_invar (queue s)"
-  assumes "Map_invar (parent s)"
+lemma list_queue_fold_cong:
+  assumes "Q_invar (queue s)"
+  assumes "P_invar (parent s)"
   assumes "distinct l"
   shows
-    "list (queue (List.fold (traverse_edge u) l s)) =
-     list (queue s) @ filter (Not \<circ> discovered s) l"
+    "Q_list (queue (List.fold (traverse_edge src u) l s)) =
+     Q_list (queue s) @ filter (Not \<circ> discovered src s) l"
   using assms
 proof (induct l arbitrary: s)
   case Nil
@@ -229,103 +248,104 @@ proof (induct l arbitrary: s)
 next
   case (Cons v vs)
   have
-    "list (queue (List.fold (traverse_edge u) (v # vs) s)) =
-     list (queue (List.fold (traverse_edge u) vs (traverse_edge u v s)))"
+    "Q_list (queue (List.fold (traverse_edge src u) (v # vs) s)) =
+     Q_list (queue (List.fold (traverse_edge src u) vs (traverse_edge src u v s)))"
     by simp
   also have
     "... =
-     list (queue (traverse_edge u v s)) @
-     filter (Not \<circ> discovered (traverse_edge u v s)) vs"
+     Q_list (queue (traverse_edge src u v s)) @
+     filter (Not \<circ> discovered src (traverse_edge src u v s)) vs"
     using Cons.prems
-    by (auto intro: invar_queue_traverse_edge invar_parent_traverse_edge Cons.hyps)
+    by (auto intro: queue_traverse_edge_invar parent_traverse_edge_invar Cons.hyps)
   also have
     "... =
-     list (queue s) @
-     (if \<not> discovered s v then [v] else []) @
-     filter (Not \<circ> discovered (traverse_edge u v s)) vs"
+     Q_list (queue s) @
+     (if \<not> discovered src s v then [v] else []) @
+     filter (Not \<circ> discovered src (traverse_edge src u v s)) vs"
     using Cons.prems(1)
     by (simp add: list_queue_traverse_edge_cong)
   also have
     "... =
-     list (queue s) @
-     (if \<not> discovered s v then [v] else []) @
-     filter (Not \<circ> discovered s) vs"
+     Q_list (queue s) @
+     (if \<not> discovered src s v then [v] else []) @
+     filter (Not \<circ> discovered src s) vs"
     using Cons.prems(2, 3)
     by (simp add: list_queue_fold_cong_aux)
-  also have "... = list (queue s) @ filter (Not \<circ> discovered s) (v # vs)"
+  also have "... = Q_list (queue s) @ filter (Not \<circ> discovered src s) (v # vs)"
     by simp
   finally show ?case
     .
 qed
 
-lemma (in bfs) list_queue_fold_cong_2:
-  assumes "G.invar (out_neighborhood (head (queue s)))"
-  assumes "Queue_invar (queue s)"
-  assumes "Map_invar (parent s)"
+lemma list_queue_fold_cong_2:
+  assumes "G.invar G"
+  assumes "Q_invar (queue s)"
+  assumes "P_invar (parent s)"
   assumes "cond s"
   shows
-    "list (queue (fold s)) =
-     list (tail (queue s)) @
-     filter (Not \<circ> discovered s) (inorder (out_neighborhood (head (queue s))))"
+    "Q_list (queue (fold G src s)) =
+     Q_list (Q_tail (queue s)) @
+     filter (Not \<circ> discovered src s) (G.out_neighborhood G (Q_head (queue s)))"
 proof -
   have
-    "list (queue (fold s)) =
-     list (queue (s\<lparr>queue := tail (queue s)\<rparr>)) @
+    "Q_list (queue (fold G src s)) =
+     Q_list (queue (s\<lparr>queue := Q_tail (queue s)\<rparr>)) @
      filter
-      (Not \<circ> discovered (s\<lparr>queue := tail (queue s)\<rparr>))
-      (inorder (out_neighborhood (head (queue s))))"
+      (Not \<circ> discovered src (s\<lparr>queue := Q_tail (queue s)\<rparr>))
+      (G.out_neighborhood G (Q_head (queue s)))"
     using assms
-    by (intro invar_tail G.inorder_distinct list_queue_fold_cong) simp+
+    by (intro tail_invar G.out_neighborhood_distinct list_queue_fold_cong) simp+
   thus ?thesis
     unfolding comp_apply
     by (simp add: discovered_def)
 qed
 
-subsubsection \<open>set \<circ> list \<circ> queue\<close>
+subsubsection \<open>@{term "set \<circ> Q_list \<circ> queue"}\<close>
 
-lemma (in bfs) queue_fold_subset_vertices:
-  assumes "Queue_invar (queue s)"
-  assumes "Map_invar (parent s)"
-  assumes "set (list (queue s)) \<subseteq> vertices"
+lemma queue_fold_subset_V:
+  assumes "G.invar G"
+  assumes "Q_invar (queue s)"
+  assumes "P_invar (parent s)"
+  assumes "set (Q_list (queue s)) \<subseteq> G.V G"
   assumes "cond s"
-  shows "set (list (queue (fold s))) \<subseteq> vertices"
+  shows "set (Q_list (queue (fold G src s))) \<subseteq> G.V G"
 proof
   fix v
-  assume assm: "v \<in> set (list (queue (fold s)))"
-  show "v \<in> vertices"
-  proof (cases "v \<in> set (filter (Not \<circ> discovered s) (inorder (out_neighborhood (head (queue s)))))")
+  assume assm: "v \<in> set (Q_list (queue (fold G src s)))"
+  show "v \<in> G.V G"
+  proof (cases "v \<in> set (filter (Not \<circ> discovered src s) (G.out_neighborhood G (Q_head (queue s))))")
     case True
-    have "G.set (out_neighborhood (head (queue s))) \<subseteq> vertices"
+    have "set (G.out_neighborhood G (Q_head (queue s))) \<subseteq> G.V G"
       using assms
-      by (intro invar_out_neighborhood_if G.out_neighborhood_subset_vertices)      
+      by (intro head_queue_mem_V G.out_neighborhood_subset_V)
     thus ?thesis
       using True
-      by (auto simp add: G.set_def)
+      by auto
   next
     case False
-    hence "v \<in> set (list (tail (queue s)))"
-      using assms assm invar_out_neighborhood_if
+    hence "v \<in> set (Q_list (Q_tail (queue s)))"
+      using assms assm
       by (auto simp add: list_queue_fold_cong_2)
-    hence "v \<in> set (list (queue s))"
-      using assms(1, 4) list_queue_non_empty
-      by (auto simp add: list_tail intro: list.set_sel(2))
+    hence "v \<in> set (Q_list (queue s))"
+      using assms(2, 5) list_queue_non_empty
+      by (auto simp add: Q.list_tail intro: list.set_sel(2))
     thus ?thesis
-      using assms(3)
+      using assms(4)
       by blast
   qed
 qed
 
-subsubsection \<open>parent\<close>
+subsubsection \<open>@{term parent}\<close>
 
-lemma (in bfs) lookup_parent_fold_cong:
-  assumes "Map_invar (parent s)"
+lemma lookup_parent_fold_cong:
+  assumes "P_invar (parent s)"
   assumes "distinct l"
   shows
-    "lookup (parent (List.fold (traverse_edge u) l s)) =
+    "P_lookup (parent (List.fold (traverse_edge src u) l s)) =
      override_on
-      (lookup (parent s))
+      (P_lookup (parent s))
       (\<lambda>_. Some u)
-      (set (filter (Not \<circ> discovered s) l))"
+      (set (filter (Not \<circ> discovered src s) l))"
   using assms
 proof (induct l arbitrary: s)
   case Nil
@@ -334,180 +354,183 @@ proof (induct l arbitrary: s)
 next
   case (Cons v vs)
   have
-    "lookup (parent (List.fold (traverse_edge u) (v # vs) s)) =
-     lookup (parent (List.fold (traverse_edge u) vs (traverse_edge u v s)))"
+    "P_lookup (parent (List.fold (traverse_edge src u) (v # vs) s)) =
+     P_lookup (parent (List.fold (traverse_edge src u) vs (traverse_edge src u v s)))"
     by simp
   also have
     "... =
      override_on
-      (lookup (parent (traverse_edge u v s)))
+      (P_lookup (parent (traverse_edge src u v s)))
       (\<lambda>_. Some u)
-      (set (filter (Not \<circ> discovered (traverse_edge u v s)) vs))"
+      (set (filter (Not \<circ> discovered src (traverse_edge src u v s)) vs))"
     using Cons.prems
-    by (fastforce intro: invar_parent_traverse_edge Cons.hyps)
+    by (fastforce intro: parent_traverse_edge_invar Cons.hyps)
   also have
     "... =
      override_on
-      (override_on (lookup (parent s)) (\<lambda>_. Some u) (if \<not> discovered s v then {v} else {}))
+      (override_on (P_lookup (parent s)) (\<lambda>_. Some u) (if \<not> discovered src s v then {v} else {}))
       (\<lambda>_. Some u)
-      (set (filter (Not \<circ> discovered (traverse_edge u v s)) vs))"
+      (set (filter (Not \<circ> discovered src (traverse_edge src u v s)) vs))"
     using Cons.prems(1)
     by (simp add: lookup_parent_traverse_edge_cong)
   also have
     "... =
      override_on
-      (override_on (lookup (parent s)) (\<lambda>_. Some u) (if \<not> discovered s v then {v} else {}))
+      (override_on (P_lookup (parent s)) (\<lambda>_. Some u) (if \<not> discovered src s v then {v} else {}))
       (\<lambda>_. Some u)
-      (set (filter (Not \<circ> discovered s) vs))"
+      (set (filter (Not \<circ> discovered src s) vs))"
     using Cons.prems
     by (simp add: list_queue_fold_cong_aux)
   finally show ?case
     by (simp add: override_on_insert')
 qed
 
-lemma (in bfs) lookup_parent_fold_cong_2:
-  assumes "G.invar (out_neighborhood (head (queue s)))"
-  assumes "Map_invar (parent s)"
+lemma lookup_parent_fold_cong_2:
+  assumes "G.invar G"
+  assumes "P_invar (parent s)"
   shows
-    "lookup (parent (fold s)) =
+    "P_lookup (parent (fold G src s)) =
      override_on
-      (lookup (parent s))
-      (\<lambda>_. Some (head (queue s)))
-      (set (filter (Not \<circ> discovered s) (inorder (out_neighborhood (head (queue s))))))"
+      (P_lookup (parent s))
+      (\<lambda>_. Some (Q_head (queue s)))
+      (set (filter (Not \<circ> discovered src s) (G.out_neighborhood G (Q_head (queue s)))))"
 proof -
   have
-    "lookup (parent (fold s)) =
+    "P_lookup (parent (fold G src s)) =
      override_on
-      (lookup (parent (s\<lparr>queue := tail (queue s)\<rparr>)))
-      (\<lambda>_. Some (head (queue s)))
-      (set (filter (Not \<circ> discovered (s\<lparr>queue := tail (queue s)\<rparr>)) (inorder (out_neighborhood (head (queue s))))))"
+      (P_lookup (parent (s\<lparr>queue := Q_tail (queue s)\<rparr>)))
+      (\<lambda>_. Some (Q_head (queue s)))
+      (set (filter (Not \<circ> discovered src (s\<lparr>queue := Q_tail (queue s)\<rparr>)) (G.out_neighborhood G (Q_head (queue s)))))"
     using assms
-    by (intro G.inorder_distinct lookup_parent_fold_cong) simp+
+    by (intro G.out_neighborhood_distinct lookup_parent_fold_cong) simp+
   thus ?thesis
     by (simp add: discovered_def)
 qed
 
-subsubsection \<open>Map_invar \<circ> parent\<close>
+subsubsection \<open>@{term "P_invar \<circ> parent"}\<close>
 
-lemma (in bfs) invar_parent_fold:
-  assumes "Map_invar (parent s)"
+lemma parent_fold_invar:
+  assumes "P_invar (parent s)"
   assumes "distinct l"
-  shows "Map_invar (parent (List.fold (traverse_edge u) l s))"
+  shows "P_invar (parent (List.fold (traverse_edge src u) l s))"
   using assms
-  by (induct l arbitrary: s) (simp_all add: invar_parent_traverse_edge)
+  by (induct l arbitrary: s) (simp_all add: parent_traverse_edge_invar)
 
-lemma (in bfs) invar_parent_fold_2:
-  assumes "G.invar (out_neighborhood (head (queue s)))"
-  assumes "Map_invar (parent s)"
-  shows "Map_invar (parent (fold s))"
+lemma parent_fold_invar_2:
+  assumes "G.invar G"
+  assumes "P_invar (parent s)"
+  shows "P_invar (parent (fold G src s))"
   using assms
-  by (intro G.inorder_distinct invar_parent_fold) simp+
+  by (intro G.out_neighborhood_distinct parent_fold_invar) simp+
 
-subsubsection \<open>dom \<circ> parent\<close>
+subsubsection \<open>@{term "P.dom \<circ> parent"}\<close>
 
-lemma (in bfs) dom_parent_fold_subset_vertices:
-  assumes "Map_invar (parent s)"
+lemma dom_parent_fold_subset_V:
+  assumes "P_invar (parent s)"
   assumes "distinct l"
-  assumes "dom (parent s) \<subseteq> vertices"
-  assumes "set l \<subseteq> vertices"
-  shows "dom (parent (List.fold (traverse_edge u) l s)) \<subseteq> vertices"
+  assumes "P.dom (parent s) \<subseteq> G.V G"
+  assumes "set l \<subseteq> G.V G"
+  shows "P.dom (parent (List.fold (traverse_edge src u) l s)) \<subseteq> G.V G"
 proof
   fix v
-  assume assm: "v \<in> dom (parent (List.fold (traverse_edge u) l s))"
-  show "v \<in> vertices"
-  proof (cases "v \<in> set (filter (Not \<circ> discovered s) l)")
+  assume assm: "v \<in> P.dom (parent (List.fold (traverse_edge src u) l s))"
+  show "v \<in> G.V G"
+  proof (cases "v \<in> set (filter (Not \<circ> discovered src s) l)")
     case True
     thus ?thesis
       using assms(4)
       by auto
   next
     case False
-    have "lookup (parent (List.fold (traverse_edge u) l s)) v \<noteq> None"
+    have "P_lookup (parent (List.fold (traverse_edge src u) l s)) v \<noteq> None"
       using assm
-      by (simp add: dom_def)
-    hence "lookup (parent s) v \<noteq> None"
+      by (simp add: P.dom_def)
+    hence "P_lookup (parent s) v \<noteq> None"
       using assms(1, 2) False
       by (simp add: lookup_parent_fold_cong)
     thus ?thesis
       using assms(3)
-      by (auto simp add: dom_def)
+      by (auto simp add: P.dom_def)
   qed
 qed
 
-lemma (in bfs) dom_parent_fold_subset_vertices_2:
-  assumes "G.invar (out_neighborhood (head (queue s)))"
-  assumes "Map_invar (parent s)"
-  assumes "dom (parent s) \<subseteq> vertices"
-  shows "dom (parent (fold s)) \<subseteq> vertices"
+lemma dom_parent_fold_subset_V_2:
+  assumes "G.invar G"
+  assumes "Q_invar (queue s)"
+  assumes "P_invar (parent s)"
+  assumes "set (Q_list (queue s)) \<subseteq> G.V G"
+  assumes "P.dom (parent s) \<subseteq> G.V G"
+  assumes "cond s"
+  shows "P.dom (parent (fold G src s)) \<subseteq> G.V G"
 proof -
-  have "G.set (out_neighborhood (head (queue s))) \<subseteq> vertices"
-    using assms(1)
-    by (intro G.out_neighborhood_subset_vertices)
+  have "set (G.out_neighborhood G (Q_head (queue s))) \<subseteq> G.V G"
+    using assms(2, 4, 6)
+    by (intro head_queue_mem_V G.out_neighborhood_subset_V)
   thus ?thesis
-    using assms G.inorder_distinct dom_parent_fold_subset_vertices
-    by (simp add: G.set_def)
+    using assms(1, 3, 5)
+    by (intro G.out_neighborhood_distinct dom_parent_fold_subset_V) simp+
 qed
 
-subsubsection \<open>ran \<circ> parent\<close>
+subsubsection \<open>@{term "P.ran \<circ> parent"}\<close>
 
-lemma (in bfs) ran_parent_fold_cong:
-  assumes "G.invar (out_neighborhood (head (queue s)))"
-  assumes "Map_invar (parent s)"
+lemma ran_parent_fold_cong:
+  assumes "G.invar G"
+  assumes "P_invar (parent s)"
   shows
-    "ran (parent (fold s)) =
-     ran (parent s) \<union>
-     (if set (filter (Not \<circ> discovered s) (inorder (out_neighborhood (head (queue s))))) = {}
+    "P.ran (parent (fold G src s)) =
+     P.ran (parent s) \<union>
+     (if set (filter (Not \<circ> discovered src s) (G.out_neighborhood G (Q_head (queue s)))) = {}
       then {}
-      else {head (queue s)})"
+      else {Q_head (queue s)})"
 proof
-  let ?S = "set (filter (Not \<circ> discovered s) (inorder (out_neighborhood (head (queue s)))))"
-  show "ran (parent (fold s)) \<subseteq> ran (parent s) \<union> (if ?S = {} then {} else {head (queue s)})"
+  let ?S = "set (filter (Not \<circ> discovered src s) (G.out_neighborhood G (Q_head (queue s))))"
+  show "P.ran (parent (fold G src s)) \<subseteq> P.ran (parent s) \<union> (if ?S = {} then {} else {Q_head (queue s)})"
     using assms
-    by (auto simp add: ran_def lookup_parent_fold_cong_2 override_on_def)
-  show "ran (parent s) \<union> (if ?S = {} then {} else {head (queue s)}) \<subseteq> ran (parent (fold s))"
+    by (auto simp add: P.ran_def lookup_parent_fold_cong_2 override_on_def)
+  show "P.ran (parent s) \<union> (if ?S = {} then {} else {Q_head (queue s)}) \<subseteq> P.ran (parent (fold G src s))"
   proof
     fix u
-    assume assm: "u \<in> ran (parent s) \<union> (if ?S = {} then {} else {head (queue s)})"
-    show "u \<in> ran (parent (fold s))"
-    proof (cases "u \<in> ran (parent s)")
+    assume assm: "u \<in> P.ran (parent s) \<union> (if ?S = {} then {} else {Q_head (queue s)})"
+    show "u \<in> P.ran (parent (fold G src s))"
+    proof (cases "u \<in> P.ran (parent s)")
       case True
       then obtain v where
-        "lookup (parent s) v = Some u"
-        by (auto simp add: ran_def)
-      moreover hence "discovered s v"
-        by (simp add: discovered_def dom_def)
+        "P_lookup (parent s) v = Some u"
+        by (auto simp add: P.ran_def)
+      moreover hence "discovered src s v"
+        by (simp add: discovered_def)
       ultimately show ?thesis
         using assms
-        by (auto simp add: ran_def lookup_parent_fold_cong_2 override_on_def)
+        by (auto simp add: P.ran_def lookup_parent_fold_cong_2 override_on_def)
     next
       case False
       then obtain v where
         "v \<in> ?S"
         using assm
         by (auto split: if_splits(2))
-      moreover have "u = head (queue s)"
+      moreover have "u = Q_head (queue s)"
         using assm False
         by (simp split: if_splits(2))
       ultimately show ?thesis
         using assms
-        by (auto simp add: ran_def lookup_parent_fold_cong_2 override_on_def)
+        by (auto simp add: P.ran_def lookup_parent_fold_cong_2 override_on_def)
     qed
   qed
 qed
 
-subsubsection \<open>@{term bfs.T}\<close>
+subsubsection \<open>@{term T}\<close>
 
-lemma (in bfs) T_fold_cong_aux:
-  assumes "Map_invar (parent s)"
+lemma T_fold_cong_aux:
+  assumes "P_invar (parent s)"
   assumes "distinct (v # vs)"
-  shows "w \<in> set vs \<and> \<not> discovered (traverse_edge u v s) w \<longleftrightarrow> w \<in> set vs \<and> \<not> discovered s w"
+  shows "w \<in> set vs \<and> \<not> discovered src (traverse_edge src u v s) w \<longleftrightarrow> w \<in> set vs \<and> \<not> discovered src s w"
   using assms
-  by (auto simp add: discovered_def dom_def lookup_parent_traverse_edge_cong override_on_def)
+  by (auto simp add: discovered_def lookup_parent_traverse_edge_cong override_on_def)
 
-lemma (in bfs) T_fold_cong:
-  assumes "Map_invar (parent s)"
+lemma T_fold_cong:
+  assumes "P_invar (parent s)"
   assumes "distinct l"
-  shows "T (List.fold (traverse_edge u) l s) = T s \<union> {(u, v) |v. v \<in> set l \<and> \<not> discovered s v}"
+  shows "T (List.fold (traverse_edge src u) l s) = T s \<union> {(u, v) |v. v \<in> set l \<and> \<not> discovered src s v}"
   using assms
 proof (induct l arbitrary: s)
   case Nil
@@ -516,152 +539,150 @@ proof (induct l arbitrary: s)
 next
   case (Cons v vs)
   have
-    "T (List.fold (traverse_edge u) (v # vs) s) =
-     T (List.fold (traverse_edge u) vs (traverse_edge u v s))"
+    "T (List.fold (traverse_edge src u) (v # vs) s) =
+     T (List.fold (traverse_edge src u) vs (traverse_edge src u v s))"
     by simp
   also have
     "... =
-     T (traverse_edge u v s) \<union>
-     {(u, w) |w. w \<in> set vs \<and> \<not> discovered (traverse_edge u v s) w}"
+     T (traverse_edge src u v s) \<union>
+     {(u, w) |w. w \<in> set vs \<and> \<not> discovered src (traverse_edge src u v s) w}"
     using Cons.prems
-    by (intro invar_parent_traverse_edge Cons.hyps) simp+
+    by (intro parent_traverse_edge_invar Cons.hyps) simp+
   also have
     "... =
      T s \<union>
-     (if \<not> discovered s v then {(u, v)} else {}) \<union>
-     {(u, w) |w. w \<in> set vs \<and> \<not> discovered (traverse_edge u v s) w}"
+     (if \<not> discovered src s v then {(u, v)} else {}) \<union>
+     {(u, w) |w. w \<in> set vs \<and> \<not> discovered src (traverse_edge src u v s) w}"
     unfolding T_traverse_edge_cong[OF Cons.prems(1)]
     by blast
   also have
     "... =
      T s \<union>
-     (if \<not> discovered s v then {(u, v)} else {}) \<union>
-     {(u, w) |w. w \<in> set vs \<and> \<not> discovered s w}"
+     (if \<not> discovered src s v then {(u, v)} else {}) \<union>
+     {(u, w) |w. w \<in> set vs \<and> \<not> discovered src s w}"
     using Cons.prems
     by (simp add: T_fold_cong_aux)
-  also have "... = T s \<union> {(u, w) |w. w \<in> set (v # vs) \<and> \<not> discovered s w}"
+  also have "... = T s \<union> {(u, w) |w. w \<in> set (v # vs) \<and> \<not> discovered src s w}"
     by force
   finally show ?case
     .
 qed
 
-lemma (in bfs) T_fold_cong_2:
-  assumes "G.invar (out_neighborhood (head (queue s)))"
-  assumes "Map_invar (parent s)"
+lemma T_fold_cong_2:
+  assumes "G.invar G"
+  assumes "P_invar (parent s)"
   shows
-    "T (fold s) =
+    "T (fold G src s) =
      T s \<union>
-     {(head (queue s), v) |v.
-      v \<in> set (inorder (out_neighborhood (head (queue s)))) \<and> \<not> discovered s v}"
+     {(Q_head (queue s), v) |v.
+      v \<in> set (G.out_neighborhood G (Q_head (queue s))) \<and> \<not> discovered src s v}"
 proof -
   have
-    "T (fold s) =
-     T (s\<lparr>queue := tail (queue s)\<rparr>) \<union>
-     {(head (queue s), v) |v.
-      v \<in> set (inorder (out_neighborhood (head (queue s)))) \<and>
-      \<not> discovered (s\<lparr>queue := tail (queue s)\<rparr>) v}"
+    "T (fold G src s) =
+     T (s\<lparr>queue := Q_tail (queue s)\<rparr>) \<union>
+     {(Q_head (queue s), v) |v.
+      v \<in> set (G.out_neighborhood G (Q_head (queue s))) \<and>
+      \<not> discovered src (s\<lparr>queue := Q_tail (queue s)\<rparr>) v}"
     using assms
-    by (intro G.inorder_distinct T_fold_cong) simp+
+    by (intro G.out_neighborhood_distinct T_fold_cong) simp+
   thus ?thesis
     by (simp add: discovered_def)
 qed
 
 section \<open>Termination\<close>
 
-lemma (in bfs) loop_dom_aux:
-  assumes "G.invar (out_neighborhood (head (queue s)))"
-  assumes "Map_invar (parent s)"
-  assumes "dom (parent s) \<subseteq> vertices"
+lemma loop_dom_aux:
+  assumes "G.invar G"
+  assumes "P_invar (parent s)"
+  assumes "P.dom (parent s) \<subseteq> G.V G"
   shows
-    "card (dom (parent (fold s))) =
-     card (dom (parent s)) +
-     card (set (filter (Not \<circ> discovered s) (inorder (out_neighborhood (head (queue s))))))"
+    "card (P.dom (parent (fold G src s))) =
+     card (P.dom (parent s)) +
+     card (set (filter (Not \<circ> discovered src s) (G.out_neighborhood G (Q_head (queue s)))))"
 proof -
-  let ?S = "set (filter (Not \<circ> discovered s) (inorder (out_neighborhood (head (queue s)))))"
-  have "dom (parent (fold s)) = dom (parent s) \<union> ?S"
+  let ?S = "set (filter (Not \<circ> discovered src s) (G.out_neighborhood G (Q_head (queue s))))"
+  have "P.dom (parent (fold G src s)) = P.dom (parent s) \<union> ?S"
     using assms(1, 2)
-    by (auto simp add: dom_def lookup_parent_fold_cong_2 override_on_def)
-  moreover have "finite (dom (parent s))"
-    using assms(3) G.vertices_finite
-    by (rule finite_subset)
+    by (auto simp add: P.dom_def lookup_parent_fold_cong_2 override_on_def)
+  moreover have "finite (P.dom (parent s))"
+    using assms(1, 3) finite_subset
+    by (fastforce intro: G.E_finite vertices_finite)
   moreover have "finite ?S"
     using G.out_neighborhood_finite
     by simp
-  moreover have "dom (parent s) \<inter> ?S = {}"
-    by (auto simp add: discovered_def)
+  moreover have "P.dom (parent s) \<inter> ?S = {}"
+    by (auto simp add: P.dom_def discovered_def)
   ultimately show ?thesis
     by (simp add: card_Un_disjoint)
 qed
 
-lemma (in bfs) loop_dom_aux_2:
-  assumes invar_queue: "Queue_invar (queue s)"
+lemma loop_dom_aux_2:
+  assumes G_invar: "G.invar G"
+  assumes queue_invar: "Q_invar (queue s)"
   assumes cond: "cond s"
-  assumes dom_parent_subset_vertices: "dom (parent s) \<subseteq> vertices"
+  assumes dom_parent_subset_V: "P.dom (parent s) \<subseteq> G.V G"
   shows
-    "card (vertices) +
-     length (list (tail (queue s))) -
-     card (dom (parent s)) <
-     card (vertices) +
-     length (list (queue s)) -
-     card (dom (parent s))"
+    "card (G.V G) +
+     length (Q_list (Q_tail (queue s))) -
+     card (P.dom (parent s)) <
+     card (G.V G) +
+     length (Q_list (queue s)) -
+     card (P.dom (parent s))"
 proof -
-  have "list (queue s) \<noteq> []"
-    using invar_queue cond
+  have "Q_list (queue s) \<noteq> []"
+    using queue_invar cond
     by (intro list_queue_non_empty)
-  hence "length (list (tail (queue s))) < length (list (queue s))"
-    using invar_queue
-    by (simp add: list_tail)
-  moreover have "card (dom (parent s)) \<le> card (vertices)"
-    using G.vertices_finite dom_parent_subset_vertices
-    by (intro card_mono)
+  hence "length (Q_list (Q_tail (queue s))) < length (Q_list (queue s))"
+    using queue_invar
+    by (simp add: Q.list_tail)
+  moreover have "card (P.dom (parent s)) \<le> card (G.V G)"
+    using G_invar dom_parent_subset_V
+    by (intro G.E_finite vertices_finite card_mono)
   ultimately show ?thesis
     by simp
 qed
 
-lemma (in bfs) loop_dom:
-  assumes "Queue_invar (queue s)"
-  assumes "Map_invar (parent s)"
-  assumes "set (list (queue s)) \<subseteq> vertices"
-  assumes "dom (parent s) \<subseteq> vertices"
-  shows "loop_dom s"
+lemma loop_dom:
+  assumes "G.invar G"
+  assumes "Q_invar (queue s)"
+  assumes "P_invar (parent s)"
+  assumes "set (Q_list (queue s)) \<subseteq> G.V G"
+  assumes "P.dom (parent s) \<subseteq> G.V G"
+  shows "loop_dom (G, src, s)"
   using assms
-proof (induct "card (vertices) + length (list (queue s)) - card (dom (parent s))"
+proof (induct "card (G.V G) + length (Q_list (queue s)) - card (P.dom (parent s))"
        arbitrary: s
        rule: less_induct)
   case less
   show ?case
   proof (cases "cond s")
     case True
-    let ?u = "head (queue s)"
-    let ?q = "tail (queue s)"
-    let ?S = "set (filter (Not \<circ> discovered s) (inorder (out_neighborhood (head (queue s)))))"
+    let ?u = "Q_head (queue s)"
+    let ?q = "Q_tail (queue s)"
+    let ?S = "set (filter (Not \<circ> discovered src s) (G.out_neighborhood G (Q_head (queue s))))"
 
-    have invar_out_neighborhood: "G.invar (out_neighborhood ?u)"
-      using less.prems(1, 3) True
-      by (rule invar_out_neighborhood_if)
-
-    hence "length (list (queue (fold s))) = length (list ?q) + card ?S"
-      using less.prems(1, 2) True G.inorder_distinct
+    have "length (Q_list (queue (fold G src s))) = length (Q_list ?q) + card ?S"
+      using less.prems(1-3) True G.out_neighborhood_distinct
       by (simp add: list_queue_fold_cong_2 distinct_card[symmetric])
-    moreover have "card (dom (parent (fold s))) = card (dom (parent s)) + card ?S"
-      using invar_out_neighborhood less.prems(2, 4)
+    moreover have "card (P.dom (parent (fold G src s))) = card (P.dom (parent s)) + card ?S"
+      using less.prems(1, 3, 5)
       by (intro loop_dom_aux)
     ultimately have
-      "card (vertices) + length (list (queue (fold s))) - card (dom (parent (fold s))) =
-       card (vertices) + length (list ?q) + card ?S - (card (dom (parent s)) + card ?S)"
+      "card (G.V G) + length (Q_list (queue (fold G src s))) - card (P.dom (parent (fold G src s))) =
+       card (G.V G) + length (Q_list ?q) + card ?S - (card (P.dom (parent s)) + card ?S)"
       by presburger
-    also have "... = card (vertices) + length (list ?q) - card (dom (parent s))"
+    also have "... = card (G.V G) + length (Q_list ?q) - card (P.dom (parent s))"
       by simp
-    also have "... < card (vertices) + length (list (queue s)) - card (dom (parent s))"
+    also have "... < card (G.V G) + length (Q_list (queue s)) - card (P.dom (parent s))"
       using less.prems True
       by (intro loop_dom_aux_2)
     finally have
-      "card (vertices) + length (list (queue (fold s))) - card (dom (parent (fold s))) <
-       card (vertices) + length (list (queue s)) - card (dom (parent s))"
+      "card (G.V G) + length (Q_list (queue (fold G src s))) - card (P.dom (parent (fold G src s))) <
+       card (G.V G) + length (Q_list (queue s)) - card (P.dom (parent s))"
       .
     thus ?thesis
-      using less.prems invar_out_neighborhood
-      by (intro invar_queue_fold_2 invar_parent_fold_2 queue_fold_subset_vertices dom_parent_fold_subset_vertices_2 less.hyps loop.domintros)
+      using less.prems
+      by (intro queue_fold_invar_2 parent_fold_invar_2 queue_fold_subset_V dom_parent_fold_subset_V_2 less.hyps loop.domintros)
   next
     case False
     thus ?thesis
@@ -669,32 +690,55 @@ proof (induct "card (vertices) + length (list (queue s)) - card (dom (parent s))
   qed
 qed
 
+end
+
 section \<open>Invariants\<close>
+
+locale bfs_invar_tbd = bfs where
+  Map_update = Map_update and
+  P_update = P_update and
+  Q_snoc = Q_snoc
+  for
+    Map_update :: "'a::linorder \<Rightarrow> 's \<Rightarrow> 'n \<Rightarrow> 'n" and
+    P_update :: "'a \<Rightarrow> 'a \<Rightarrow> 'm \<Rightarrow> 'm" and
+    Q_snoc :: "'q \<Rightarrow> 'a \<Rightarrow> 'q" +
+  fixes G :: 'n
+  fixes src :: 'a
+  assumes G_invar: "G.invar G"
+  assumes src_mem_V: "src \<in> G.V G"
+begin
+
+subsection \<open>Convenience Lemmas\<close>
+
+lemma E_finite:
+  shows "finite (G.E G)"
+  using G_invar
+  by (intro G.E_finite)
 
 subsection \<open>\<close>
 
-abbreviation (in bfs) white :: "('q, 'm) state \<Rightarrow> 'a \<Rightarrow> bool" where
-  "white s v \<equiv> \<not> discovered s v"
+abbreviation white :: "('q, 'm) state \<Rightarrow> 'a \<Rightarrow> bool" where
+  "white s v \<equiv> \<not> discovered src s v"
 
-abbreviation (in bfs) gray :: "('q, 'm) state \<Rightarrow> 'a \<Rightarrow> bool" where
-  "gray s v \<equiv> discovered s v \<and> v \<in> set (list (queue s))"
+abbreviation gray :: "('q, 'm) state \<Rightarrow> 'a \<Rightarrow> bool" where
+  "gray s v \<equiv> discovered src s v \<and> v \<in> set (Q_list (queue s))"
 
-lemma (in bfs) gray_imp_not_white:
+abbreviation black :: "('q, 'm) state \<Rightarrow> 'a \<Rightarrow> bool" where
+  "black s v \<equiv> discovered src s v \<and> v \<notin> set (Q_list (queue s))"
+
+lemma gray_imp_not_white:
   assumes "gray s v"
   shows "\<not> white s v"
   using assms
   by simp
 
-abbreviation (in bfs) black :: "('q, 'm) state \<Rightarrow> 'a \<Rightarrow> bool" where
-  "black s v \<equiv> discovered s v \<and> v \<notin> set (list (queue s))"
-
-lemma (in bfs) black_imp_not_white:
+lemma black_imp_not_white:
   assumes "black s v"
   shows "\<not> white s v"
   using assms
   by simp
 
-lemma (in bfs) vertex_color_induct [case_names white gray black]:
+lemma vertex_color_induct [case_names white gray black]:
   assumes "white s v \<Longrightarrow> P s v"
   assumes "gray s v \<Longrightarrow> P s v"
   assumes "black s v \<Longrightarrow> P s v"
@@ -702,176 +746,177 @@ lemma (in bfs) vertex_color_induct [case_names white gray black]:
   using assms
   by blast
 
+end
+
 locale bfs_invar =
-  bfs where update = update and snoc = snoc +
-  parent "lookup (parent s)"
+  bfs_invar_tbd where P_update = P_update and Q_snoc = Q_snoc +
+  parent "P_lookup (parent s)"
   for
-    update :: "'a::linorder \<Rightarrow> 'a \<Rightarrow> 'm \<Rightarrow> 'm" and
-    snoc :: "'q \<Rightarrow> 'a \<Rightarrow> 'q" and
+    P_update :: "'a::linorder \<Rightarrow> 'a \<Rightarrow> 'm \<Rightarrow> 'm" and
+    Q_snoc :: "'q \<Rightarrow> 'a \<Rightarrow> 'q" and
     s :: "('q, 'm) state" +
-  assumes invar_queue: "Queue_invar (queue s)"
-  assumes queue_distinct: "distinct (list (queue s))"
-  assumes invar_parent: "Map_invar (parent s)"
-  assumes parent_src: "lookup (parent s) src = None"
-  assumes gray_if_mem_queue: "v \<in> set (list (queue s)) \<Longrightarrow> gray s v"
-  assumes black_if_mem_ran: "v \<in> ran (parent s) \<Longrightarrow> black s v"
+  assumes queue_invar: "Q_invar (queue s)"
+  assumes queue_distinct: "distinct (Q_list (queue s))"
+  assumes parent_invar: "P_invar (parent s)"
+  assumes parent_src: "P_lookup (parent s) src = None"
+  assumes gray_if_mem_queue: "v \<in> set (Q_list (queue s)) \<Longrightarrow> gray s v"
+  assumes black_if_mem_ran: "v \<in> P.ran (parent s) \<Longrightarrow> black s v"
   assumes queue_sorted_wrt_dpath_length:
-    "sorted_wrt (\<lambda>u v. dpath_length (rev (follow u)) \<le> dpath_length (rev (follow v))) (list (queue s))"
+    "sorted_wrt (\<lambda>u v. dpath_length (rev (follow u)) \<le> dpath_length (rev (follow v))) (Q_list (queue s))"
   assumes tbd_dpath_length:
-    "\<not> is_empty (queue s) \<Longrightarrow>
-     dpath_length (rev (follow (last (list (queue s))))) \<le> dpath_length (rev (follow (head (queue s)))) + 1"
+    "\<not> Q_is_empty (queue s) \<Longrightarrow>
+     dpath_length (rev (follow (last (Q_list (queue s))))) \<le> dpath_length (rev (follow (Q_head (queue s)))) + 1"
   assumes not_white_imp_shortest_dpath:
-    "\<not> white s v \<Longrightarrow> dpath_bet edges (rev (follow v)) src v \<and> dpath_length (rev (follow v)) = dist v"
-  assumes black_imp_out_neighborhood_not_white: "black s v \<Longrightarrow> \<forall>w\<in>G.set (out_neighborhood v). \<not> white s w"
+    "\<not> white s v \<Longrightarrow> is_shortest_dpath G (rev (follow v)) src v"
+  assumes black_imp_out_neighborhood_not_white: "black s v \<Longrightarrow> \<forall>w\<in>set (G.out_neighborhood G v). \<not> white s w"
+begin
 
 subsection \<open>Convenience Lemmas\<close>
 
-lemma (in bfs_invar) queue_subset_vertices:
-  shows "set (list (queue s)) \<subseteq> vertices"
+lemma queue_subset_V:
+  shows "set (Q_list (queue s)) \<subseteq> G.V G"
   using gray_if_mem_queue not_white_imp_shortest_dpath
-  by (auto simp add: G.vertices_eq_dVs[symmetric] intro: dpath_bet_endpoints(2))
+  by (fastforce intro: dpath_bet_endpoints(2))
 
-lemma (in bfs_invar) invar_out_neighborhood:
+lemma head_queue_mem_V:
   assumes "cond s"
-  shows "G.invar (out_neighborhood (head (queue s)))"
-  using invar_queue queue_subset_vertices assms
-  by (intro invar_out_neighborhood_if)
+  shows "Q_head (queue s) \<in> G.V G"
+  using queue_invar assms queue_subset_V
+  by (intro head_queue_mem_V)
 
-lemma (in bfs_invar) list_queue_fold_cong:
-  assumes "cond s"
-  shows
-    "list (queue (fold s)) =
-     list (tail (queue s)) @
-     filter (Not \<circ> discovered s) (inorder (out_neighborhood (head (queue s))))"
-  using invar_queue invar_parent assms
-  by (intro invar_out_neighborhood list_queue_fold_cong_2)
-
-lemma (in bfs_invar) lookup_parent_fold_cong:
+lemma list_queue_fold_cong:
   assumes "cond s"
   shows
-    "lookup (parent (fold s)) =
+    "Q_list (queue (fold G src s)) =
+     Q_list (Q_tail (queue s)) @
+     filter (Not \<circ> discovered src s) (G.out_neighborhood G (Q_head (queue s)))"
+  using G_invar queue_invar parent_invar assms
+  by (intro list_queue_fold_cong_2)
+
+lemma lookup_parent_fold_cong:
+  shows
+    "P_lookup (parent (fold G src s)) =
      override_on
-      (lookup (parent s))
-      (\<lambda>_. Some (head (queue s)))
-      (set (filter (Not \<circ> discovered s) (inorder (out_neighborhood (head (queue s))))))"
-  using assms invar_parent
-  by (intro invar_out_neighborhood lookup_parent_fold_cong_2)
+      (P_lookup (parent s))
+      (\<lambda>_. Some (Q_head (queue s)))
+      (set (filter (Not \<circ> discovered src s) (G.out_neighborhood G (Q_head (queue s)))))"
+  using G_invar parent_invar
+  by (intro lookup_parent_fold_cong_2)
 
-lemma (in bfs_invar) T_fold_cong:
-  assumes "cond s"
+lemma T_fold_cong:
   shows
-    "T (fold s) =
+    "T (fold G src s) =
      T s \<union>
-     {(head (queue s), v) |v.
-      v \<in> set (inorder (out_neighborhood (head (queue s)))) \<and> \<not> discovered s v}"
-  using assms invar_parent
-  by (intro invar_out_neighborhood T_fold_cong_2)
+     {(Q_head (queue s), v) |v.
+      v \<in> set (G.out_neighborhood G (Q_head (queue s))) \<and> \<not> discovered src s v}"
+  using G_invar parent_invar
+  by (intro T_fold_cong_2)
 
-lemma (in bfs_invar) src_not_white:
+lemma src_not_white:
   shows "\<not> white s src"
   by (simp add: discovered_def)
 
-lemma (in bfs_invar) mem_queue_imp_dpath_length_head_queue:
-  assumes "v \<in> set (list (queue s))"
-  shows "dpath_length (rev (follow (head (queue s)))) \<le> dpath_length (rev (follow v))"
-proof (cases "v = head (queue s)")
+lemma mem_queue_imp_dpath_length_head_queue:
+  assumes "v \<in> set (Q_list (queue s))"
+  shows "dpath_length (rev (follow (Q_head (queue s)))) \<le> dpath_length (rev (follow v))"
+proof (cases "v = Q_head (queue s)")
   case True
   thus ?thesis
     by simp
 next
   case False
-  have "\<not> is_empty (queue s)"
-    using invar_queue assms
-    by (auto simp add: is_empty)
-  moreover hence "head (queue s) = hd (list (queue s))"
-    using invar_queue list_head
-    by (simp add: is_empty)
+  have "\<not> Q_is_empty (queue s)"
+    using queue_invar assms
+    by (auto simp add: Q.is_empty)
+  moreover hence "Q_head (queue s) = hd (Q_list (queue s))"
+    using queue_invar Q.list_head
+    by (simp add: Q.is_empty)
   ultimately show ?thesis
     using queue_sorted_wrt_dpath_length assms False sorted_wrt_imp_hd
     by fastforce
 qed
 
-lemma (in bfs_invar) mem_queue_imp_dist_head_queue:
-  assumes "v \<in> set (list (queue s))"
-  shows "dist (head (queue s)) \<le> dist v"
+lemma mem_queue_imp_dist_head_queue:
+  assumes "v \<in> set (Q_list (queue s))"
+  shows "dist G src (Q_head (queue s)) \<le> dist G src v"
 proof -
-  have "list (queue s) \<noteq> []"
+  have "Q_list (queue s) \<noteq> []"
     using assms
     by fastforce
-  hence "head (queue s) \<in> set (list (queue s))"
-    using invar_queue
-    by (simp add: list_head)
-  hence "dist (head (queue s)) = dpath_length (rev (follow (head (queue s))))"
-    using gray_if_mem_queue
-    by (simp add: not_white_imp_shortest_dpath)
+  hence "Q_head (queue s) \<in> set (Q_list (queue s))"
+    using queue_invar
+    by (simp add: Q.list_head)
+  hence "dist G src (Q_head (queue s)) = dpath_length (rev (follow (Q_head (queue s))))"
+    using gray_if_mem_queue not_white_imp_shortest_dpath
+    by force
   also have "... \<le> dpath_length (rev (follow v))"
     using assms
     by (auto intro: mem_queue_imp_dpath_length_head_queue)
-  also have "... = dist v"
+  also have "... = dist G src v"
     using assms gray_if_mem_queue
     by (simp add: not_white_imp_shortest_dpath)
   finally show ?thesis
     .
 qed
 
-lemma (in bfs_invar) mem_queue_imp_dpath_length_last_queue:
-  assumes "v \<in> set (list (queue s))"
-  shows "dpath_length (rev (follow v)) \<le> dpath_length (rev (follow (last (list (queue s)))))"
-proof (cases "v = last (list (queue s))")
+lemma mem_queue_imp_dpath_length_last_queue:
+  assumes "v \<in> set (Q_list (queue s))"
+  shows "dpath_length (rev (follow v)) \<le> dpath_length (rev (follow (last (Q_list (queue s)))))"
+proof (cases "v = last (Q_list (queue s))")
   case True
   thus ?thesis
     by simp
 next
   case False
-  have "\<not> is_empty (queue s)"
-    using invar_queue assms
-    by (auto simp add: is_empty)
+  have "\<not> Q_is_empty (queue s)"
+    using queue_invar assms
+    by (auto simp add: Q.is_empty)
   thus ?thesis
     using queue_sorted_wrt_dpath_length assms False sorted_wrt_imp_last
     by fastforce
 qed
 
-lemma (in bfs_invar) mem_queue_imp_dist_last_queue:
-  assumes "v \<in> set (list (queue s))"
-  shows "dist v \<le> dist (last (list (queue s)))"
+lemma mem_queue_imp_dist_last_queue:
+  assumes "v \<in> set (Q_list (queue s))"
+  shows "dist G src v \<le> dist G src (last (Q_list (queue s)))"
 proof -
-  have list_queue_non_empty: "list (queue s) \<noteq> []"
+  have list_queue_non_empty: "Q_list (queue s) \<noteq> []"
     using assms
     by fastforce
-  have "dist v = dpath_length (rev (follow v))"
-    using assms gray_if_mem_queue
-    by (simp add: not_white_imp_shortest_dpath)
-  also have "... \<le> dpath_length (rev (follow (last (list (queue s)))))"
+  have "dist G src v = dpath_length (rev (follow v))"
+    using assms gray_if_mem_queue not_white_imp_shortest_dpath
+    by force
+  also have "... \<le> dpath_length (rev (follow (last (Q_list (queue s)))))"
     using assms
     by (auto intro: mem_queue_imp_dpath_length_last_queue)
-  also have "... = dist (last (list (queue s)))"
+  also have "... = dist G src (last (Q_list (queue s)))"
     using list_queue_non_empty gray_if_mem_queue
     by (simp add: not_white_imp_shortest_dpath)
   finally show ?thesis
     .
 qed
 
-lemma (in bfs_invar) mem_queue_dpath_lengthI:
-  assumes "v \<in> set (list (queue s))"
+lemma mem_queue_dpath_lengthI:
+  assumes "v \<in> set (Q_list (queue s))"
   shows
-    "dpath_length (rev (follow (head (queue s)))) \<le> dpath_length (rev (follow v))"
-    "dpath_length (rev (follow v)) \<le> dpath_length (rev (follow (last (list (queue s)))))"
+    "dpath_length (rev (follow (Q_head (queue s)))) \<le> dpath_length (rev (follow v))"
+    "dpath_length (rev (follow v)) \<le> dpath_length (rev (follow (last (Q_list (queue s)))))"
   using assms
   by (auto intro: mem_queue_imp_dpath_length_head_queue mem_queue_imp_dpath_length_last_queue)
 
-lemma (in bfs_invar) mem_queue_distI:
-  assumes "v \<in> set (list (queue s))"
+lemma mem_queue_distI:
+  assumes "v \<in> set (Q_list (queue s))"
   shows
-    "dist (head (queue s)) \<le> dist v"
-    "dist v \<le> dist (last (list (queue s)))"
+    "dist G src (Q_head (queue s)) \<le> dist G src v"
+    "dist G src v \<le> dist G src (last (Q_list (queue s)))"
   using assms
   by (auto intro: mem_queue_imp_dist_head_queue mem_queue_imp_dist_last_queue)
 
 subsection \<open>Basic Lemmas\<close>
 
-lemma (in bfs_invar) parent_imp_edge:
-  assumes "lookup (parent s) v = Some u"
-  shows "(u, v) \<in> edges"
+lemma parent_imp_edge:
+  assumes "P_lookup (parent s) v = Some u"
+  shows "(u, v) \<in> (G.E G)"
 proof -
   have "rev (follow v) = rev (follow u) @ [v]"
     using assms
@@ -881,66 +926,67 @@ proof -
     by metis
   ultimately have "rev (follow v) = rev (tl (follow u)) @ [u, v]"
     by simp
-  moreover have "dpath_bet edges (rev (follow v)) src v"
+  moreover have "dpath_bet (G.E G) (rev (follow v)) src v"
     using assms not_white_imp_shortest_dpath
-    by (simp add: discovered_def dom_def)
-  ultimately have "dpath_bet edges (rev (tl (follow u)) @ [u, v]) src v"
+    thm discovered_def
+    by (simp add: discovered_def)
+  ultimately have "dpath_bet (G.E G) (rev (tl (follow u)) @ [u, v]) src v"
     by simp
   thus ?thesis
     by (auto simp add: edge_iff_dpath_bet intro: split_dpath)
 qed
 
-lemma (in bfs_invar) dom_parent_subset_vertices:
-  shows "dom (parent s) \<subseteq> vertices"
+lemma dom_parent_subset_V:
+  shows "P.dom (parent s) \<subseteq> G.V G"
 proof
   fix v
-  assume "v \<in> dom (parent s)"
+  assume "v \<in> P.dom (parent s)"
   then obtain u where
-    "lookup (parent s) v = Some u"
-    by (auto simp add: dom_def)
-  hence "(u, v) \<in> edges"
+    "P_lookup (parent s) v = Some u"
+    by (auto simp add: P.dom_def)
+  hence "(u, v) \<in> (G.E G)"
     by (intro parent_imp_edge)
-  thus "v \<in> vertices"
+  thus "v \<in> G.V G"
     by (intro G.edgeI(2))
 qed
 
-lemma (in bfs_invar) queue_sorted_wrt_dist:
-  shows "sorted_wrt (\<lambda>u v. dist u \<le> dist v) (list (queue s))"
+lemma queue_sorted_wrt_dist:
+  shows "sorted_wrt (\<lambda>u v. dist G src u \<le> dist G src v) (Q_list (queue s))"
 proof -
-  have "\<forall>v\<in>set (list (queue s)). dpath_length (rev (follow v)) = dist v"
+  have "\<forall>v\<in>set (Q_list (queue s)). dpath_length (rev (follow v)) = dist G src v"
     using gray_if_mem_queue not_white_imp_shortest_dpath
     by blast
   hence
-    "\<And>u v. u \<in> set (list (queue s)) \<Longrightarrow>
-            v \<in> set (list (queue s)) \<Longrightarrow>
+    "\<And>u v. u \<in> set (Q_list (queue s)) \<Longrightarrow>
+            v \<in> set (Q_list (queue s)) \<Longrightarrow>
             dpath_length (rev (follow u)) \<le> dpath_length (rev (follow v)) \<Longrightarrow>
-            (\<lambda>u v. dist u \<le> dist v) u v"
+            (\<lambda>u v. dist G src u \<le> dist G src v) u v"
     by (simp add: enat_ord_simps(1)[symmetric])
   thus ?thesis
-    using queue_sorted_wrt_dpath_length sorted_wrt_mono_rel[of "(list (queue s))"]
+    using queue_sorted_wrt_dpath_length sorted_wrt_mono_rel[of "(Q_list (queue s))"]
     by presburger
 qed
 
-lemma (in bfs_invar) tbd_dist:
-  assumes "\<not> is_empty (queue s)"
-  shows "dist (last (list (queue s))) \<le> dist (head (queue s)) + 1"
+lemma tbd_dist:
+  assumes "\<not> Q_is_empty (queue s)"
+  shows "dist G src (last (Q_list (queue s))) \<le> dist G src (Q_head (queue s)) + 1"
 proof -
-  have "\<forall>v\<in>set (list (queue s)). dpath_length (rev (follow v)) = dist v"
+  have "\<forall>v\<in>set (Q_list (queue s)). dpath_length (rev (follow v)) = dist G src v"
     using gray_if_mem_queue not_white_imp_shortest_dpath
     by blast
   moreover have
-    "last (list (queue s)) \<in> set (list (queue s))"
-    "head (queue s) \<in> set (list (queue s))"
-    using invar_queue assms
-    by (simp_all add: is_empty list_head)
+    "last (Q_list (queue s)) \<in> set (Q_list (queue s))"
+    "Q_head (queue s) \<in> set (Q_list (queue s))"
+    using queue_invar assms
+    by (simp_all add: Q.is_empty Q.list_head)
   ultimately show ?thesis
     using assms tbd_dpath_length
     unfolding enat_ord_simps(1)[symmetric] plus_enat_simps(1)[symmetric] one_enat_def[symmetric]
     by simp
 qed
 
-lemma (in bfs_invar) white_imp_gray_ancestor:
-  assumes "dpath_bet edges p u v"
+lemma white_imp_gray_ancestor:
+  assumes "dpath_bet (G.E G) p u v"
   assumes "\<not> white s u"
   assumes "white s v"
   shows "\<exists>v\<in>set p. gray s v"
@@ -961,7 +1007,7 @@ next
   show ?case
   proof (induct s w rule: vertex_color_induct)
     case white
-    have "dpath_bet edges (l @ [w]) u w"
+    have "dpath_bet (G.E G) (l @ [w]) u w"
       using "3.prems"(1)
       by (intro dpath_bet_pref) simp
     hence "\<exists>v\<in>set (l @ [w]). gray s v"
@@ -975,9 +1021,9 @@ next
       by simp
   next
     case black
-    have "v \<in> G.set (out_neighborhood w)"
+    have "v \<in> set (G.out_neighborhood G w)"
       using "3.prems"(1)
-      by (auto simp add: dpath_bet_def intro: dpath_snoc_edge_2 G.mem_out_neighborhood_if_edge)
+      by (auto simp add: dpath_bet_def G.mem_out_neighborhood_iff_edge intro: dpath_snoc_edge_2)
     hence "\<not> white s v"
       using black black_imp_out_neighborhood_not_white
       by blast
@@ -987,30 +1033,30 @@ next
   qed
 qed
 
-lemma (in bfs_invar) white_imp_dist_ge_case_1_subcase_3:
+lemma white_imp_dist_ge_case_1_subcase_3:
   assumes IH:
-    "\<And>v. \<lbrakk> dpath_bet edges (l @ [u]) src v \<and> dpath_length (l @ [u]) = dist v; white s v \<rbrakk> \<Longrightarrow>
-          (if is_empty (queue s) then \<infinity> else dist (last (list (queue s)))) \<le> dist v"
-  assumes shortest_dpath: "dpath_bet edges (l @ [u, u']) src v \<and> dpath_length (l @ [u, u']) = dist v"
+    "\<And>v. \<lbrakk> dpath_bet (G.E G) (l @ [u]) src v \<and> dpath_length (l @ [u]) = dist G src v; white s v \<rbrakk> \<Longrightarrow>
+          (if Q_is_empty (queue s) then \<infinity> else dist G src (last (Q_list (queue s)))) \<le> dist G src v"
+  assumes shortest_dpath: "is_shortest_dpath G (l @ [u, u']) src v"
   assumes white: "white s v"
-  shows "(if is_empty (queue s) then \<infinity> else dist (last (list (queue s)))) \<le> dist v"
+  shows "(if Q_is_empty (queue s) then \<infinity> else dist G src (last (Q_list (queue s)))) \<le> dist G src v"
 proof (induct s u rule: vertex_color_induct)
   case white
-  have l_snoc_u_shortest_dpath: "dpath_bet edges (l @ [u]) src u \<and> dpath_length (l @ [u]) = dist u"
-    using shortest_dpath
+  have l_Q_snoc_u_shortest_dpath: "is_shortest_dpath G (l @ [u]) src u"
+    using G_invar shortest_dpath
     by
       (auto
-       simp add: dpath_length_eq_dpath_weight dist_eq_\<delta> is_shortest_dpath_def[symmetric]
-       intro: G.G.shortest_dpath_prefix_is_shortest_dpath)
-  hence "(if is_empty (queue s) then \<infinity> else dist (last (list (queue s)))) \<le> dist u"
+        simp add: dpath_length_eq_dpath_weight dist_eq_\<delta> is_shortest_dpath_def[symmetric]
+        intro: G.E_finite shortest_dpath_prefix_is_shortest_dpath)
+  hence "(if Q_is_empty (queue s) then \<infinity> else dist G src (last (Q_list (queue s)))) \<le> dist G src u"
     using white
     by (intro IH)
   also have "... = dpath_length (l @ [u])"
-    by (simp add: l_snoc_u_shortest_dpath)
+    by (simp add: l_Q_snoc_u_shortest_dpath)
   also have "... \<le> dpath_length (l @ [u, u'])"
     using dpath_length_append[where ?p = "l @ [u]" and ?q = "[u']"]
     by simp
-  also have "... = dist v"
+  also have "... = dist G src v"
     by (simp add: shortest_dpath)
   finally show ?case
     .
@@ -1019,25 +1065,25 @@ next
   hence "\<exists>v\<in>set (l @ [u, u']). gray s v"
     using src_not_white shortest_dpath white
     by (blast intro: white_imp_gray_ancestor)
-  hence queue_non_empty: "\<not> is_empty (queue s)"
-    using invar_queue
-    by (auto simp add: is_empty)
-  hence "dist (last (list (queue s))) \<le> dist (head (queue s)) + 1"
+  hence queue_non_empty: "\<not> Q_is_empty (queue s)"
+    using queue_invar
+    by (auto simp add: Q.is_empty)
+  hence "dist G src (last (Q_list (queue s))) \<le> dist G src (Q_head (queue s)) + 1"
     by (intro tbd_dist)
-  also have "... \<le> dist u + 1"
+  also have "... \<le> dist G src u + 1"
     using gray
     by (blast intro: mem_queue_imp_dist_head_queue add_right_mono)
-  also have "... = dist v"
-    using shortest_dpath
-    by (auto intro: G.G.shortest_dpathE_2)
+  also have "... = dist G src v"
+    using G_invar shortest_dpath
+    by (auto intro: G.E_finite shortest_dpathE_2)
   finally show ?case
     using queue_non_empty
     by simp
 next
   case black
-  have "v \<in> G.set (out_neighborhood u)"
+  have "v \<in> set (G.out_neighborhood G u)"
     using shortest_dpath
-    by (auto simp add: dpath_bet_def intro: dpath_snoc_edge_2 G.mem_out_neighborhood_if_edge)
+    by (auto simp add: dpath_bet_def G.mem_out_neighborhood_iff_edge intro: dpath_snoc_edge_2)
   hence "\<not> white s v"
     using black black_imp_out_neighborhood_not_white
     by blast
@@ -1046,14 +1092,15 @@ next
     by simp
 qed
 
-lemma (in bfs_invar) white_imp_dist_ge:
+lemma white_imp_dist_ge:
   assumes "white s v"
-  shows "(if is_empty (queue s) then \<infinity> else dist (last (list (queue s)))) \<le> dist v"
-proof (cases "reachable edges src v")
+  shows "(if Q_is_empty (queue s) then \<infinity> else dist G src (last (Q_list (queue s)))) \<le> dist G src v"
+proof (cases "reachable (G.E G) src v")
   case True
   then obtain p where
-    "dpath_bet edges p src v \<and> dpath_length p = dist v"
-    by (elim G.G.dist_dpath_betE) simp
+    "dpath_bet (G.E G) p src v \<and> dpath_length p = dist G src v"
+    using E_finite
+    by (elim dist_dpath_betE) simp+
   thus ?thesis
     using assms
   proof (induct p arbitrary: v rule: dpath_rev_induct)
@@ -1074,116 +1121,137 @@ proof (cases "reachable edges src v")
   qed
 next
   case False
-  hence "dist v = \<infinity>"
+  hence "dist G src v = \<infinity>"
     unfolding dist_eq_\<delta>
     by (meson \<delta>_reachable_conv)
   thus ?thesis
     by simp
 qed
 
+end
+
+abbreviation (in bfs) bfs_invar_tbd' :: "'n \<Rightarrow> 'a \<Rightarrow> bool"  where
+  "bfs_invar_tbd' G src \<equiv>
+   bfs_invar_tbd
+    Map_empty Map_delete Map_lookup Map_inorder Map_inv
+    Set_empty Set_insert Set_delete Set_isin Set_inorder Set_inv
+    P_empty P_delete P_lookup P_invar
+    Q_empty Q_is_empty Q_head Q_tail Q_invar Q_list
+    Map_update P_update Q_snoc G src"
+
+abbreviation (in bfs) bfs_invar' :: "'n \<Rightarrow> 'a \<Rightarrow> ('q, 'm) state \<Rightarrow> bool"  where
+  "bfs_invar' G src s \<equiv>
+   bfs_invar
+    Map_empty Map_delete Map_lookup Map_inorder Map_inv
+    Set_empty Set_insert Set_delete Set_isin Set_inorder Set_inv
+    P_empty P_delete P_lookup P_invar
+    Q_empty Q_is_empty Q_head Q_tail Q_invar Q_list
+    Map_update G src P_update Q_snoc s"
+
+abbreviation (in bfs_invar_tbd) bfs_invar'' :: "('q, 'm) state \<Rightarrow> bool"  where
+  "bfs_invar'' \<equiv> bfs_invar' G src"
+
 subsection \<open>@{term bfs.init}\<close>
 
 subsubsection \<open>\<close>
 
-lemma (in bfs) follow_invar'_parent_init:
-  shows "follow_invar' (lookup (parent init))"
+lemma (in bfs_invar_tbd) follow_invar'_parent_init:
+  shows "follow_invar' (P_lookup (parent (init src)))"
   using wf_empty
-  by (simp add: init_def map_empty follow_invar'_def)
+  by (simp add: init_def P.map_empty follow_invar'_def)
 
-lemma (in bfs) parent_init:
-  shows "Tbd.parent (lookup (parent init))"
+lemma (in bfs_invar_tbd) parent_init:
+  shows "Tbd.parent (P_lookup (parent (init src)))"
   using follow_invar'_parent_init
   by unfold_locales
 
-subsubsection \<open>@{thm bfs_invar.invar_queue}\<close>
+subsubsection \<open>@{thm bfs_invar.queue_invar}\<close>
 
-lemma (in bfs) invar_queue_init:
-  shows "Queue_invar (queue init)"
-  using invar_empty
-  by (auto simp add: init_def intro: invar_snoc)
+lemma (in bfs_invar_tbd) queue_invar_init:
+  shows "Q_invar (queue (init src))"
+  using Q.invar_empty
+  by (auto simp add: init_def intro: Q.invar_snoc)
 
 subsubsection \<open>@{thm bfs_invar.queue_distinct}\<close>
 
-lemma (in bfs) queue_distinct_init:
-  shows "distinct (list (queue init))"
-  using invar_empty
-  by (simp add: init_def list_snoc list_empty)
+lemma (in bfs_invar_tbd) queue_distinct_init:
+  shows "distinct (Q_list (queue (init src)))"
+  using Q.invar_empty
+  by (simp add: init_def Q.list_snoc Q.list_empty)
 
-subsubsection \<open>@{thm bfs_invar.invar_parent}\<close>
+subsubsection \<open>@{thm bfs_invar.parent_invar}\<close>
 
-lemma (in bfs) invar_parent_init:
-  shows "Map_invar (parent init)"
-  using map_specs(4)
+lemma (in bfs_invar_tbd) parent_invar_init:
+  shows "P_invar (parent (init src))"
+  using P.map_specs(4)
   by (simp add: init_def)
 
 subsubsection \<open>@{thm bfs_invar.parent_src}\<close>
 
-lemma (in bfs) parent_src_init:
-  shows "lookup (parent init) src = None"
-  by (simp add: init_def map_empty)
+lemma (in bfs_invar_tbd) parent_src_init:
+  shows "P_lookup (parent (init src)) src = None"
+  by (simp add: init_def P.map_empty)
 
 subsubsection \<open>@{thm bfs_invar.gray_if_mem_queue}\<close>
 
-lemma (in bfs) gray_if_mem_queue_init:
-  assumes "v \<in> set (list (queue init))"
-  shows "gray init v"
-  using assms invar_empty
-  by (simp add: init_def list_snoc list_empty discovered_def)
+lemma (in bfs_invar_tbd) gray_if_mem_queue_init:
+  assumes "v \<in> set (Q_list (queue (init src)))"
+  shows "gray (init src) v"
+  using assms Q.invar_empty
+  by (simp add: init_def Q.list_snoc Q.list_empty discovered_def)
 
 subsubsection \<open>@{thm bfs_invar.black_if_mem_ran}\<close>
 
-lemma (in bfs) black_if_mem_ran_init:
-  assumes "v \<in> ran (parent init)"
-  shows "black init v"
+lemma (in bfs_invar_tbd) black_if_mem_ran_init:
+  assumes "v \<in> P.ran (parent (init src))"
+  shows "black (init src) v"
   using assms
-  by (simp add: init_def ran_def map_empty)
+  by (simp add: init_def P.ran_def P.map_empty)
 
 subsubsection \<open>@{thm bfs_invar.queue_sorted_wrt_dpath_length}\<close>
 
-lemma (in bfs) queue_sorted_wrt_dpath_length_init:
+lemma (in bfs_invar_tbd) queue_sorted_wrt_dpath_length_init:
   shows
     "sorted_wrt
-      (\<lambda>u v. dpath_length (rev (parent.follow (lookup (parent init)) u)) \<le>
-             dpath_length (rev (parent.follow (lookup (parent init)) v)))
-      (list (queue init))"
-  using invar_empty
-  by (simp add: init_def list_snoc list_empty)
+      (\<lambda>u v. dpath_length (rev (parent.follow (P_lookup (parent (init src))) u)) \<le>
+             dpath_length (rev (parent.follow (P_lookup (parent (init src))) v)))
+      (Q_list (queue (init src)))"
+  using Q.invar_empty
+  by (simp add: init_def Q.list_snoc Q.list_empty)
 
 subsubsection \<open>@{thm bfs_invar.tbd_dpath_length}\<close>
 
-lemma (in bfs) tbd_dpath_length_init:
-  assumes "\<not> is_empty (queue init)"
+lemma (in bfs_invar_tbd) tbd_dpath_length_init:
+  assumes "\<not> Q_is_empty (queue (init src))"
   shows
-    "dpath_length (rev (parent.follow (lookup (parent init)) (last (list (queue init))))) \<le>
-     dpath_length (rev (parent.follow (lookup (parent init)) (head (queue init)))) + 1"
-  using invar_empty invar_queue_init
-  by (simp add: init_def list_snoc list_empty list_head)
+    "dpath_length (rev (parent.follow (P_lookup (parent (init src))) (last (Q_list (queue (init src)))))) \<le>
+     dpath_length (rev (parent.follow (P_lookup (parent (init src))) (Q_head (queue (init src))))) + 1"
+  using Q.invar_empty queue_invar_init
+  by (simp add: init_def Q.list_snoc Q.list_empty Q.list_head)
 
 subsubsection \<open>@{thm bfs_invar.not_white_imp_shortest_dpath}\<close>
 
-lemma (in bfs) not_white_imp_shortest_dpath_init:
-  assumes "\<not> white init v"
-  shows
-    "dpath_bet edges (rev (parent.follow (lookup (parent init)) v)) src v \<and>
-     dpath_length (rev (parent.follow (lookup (parent init)) v)) = dist v"
+lemma (in bfs_invar_tbd) not_white_imp_shortest_dpath_init:
+  assumes "\<not> white (init src) v"
+  shows "is_shortest_dpath G (rev (parent.follow (P_lookup (parent (init src))) v)) src v"
 proof -
-  have dpath_bet: "dpath_bet edges [src] src src"
-    using src_mem_vertices
-    by (auto simp add: G.vertices_eq_dVs intro: dpath_bet_reflexive)
+  have dpath_bet: "dpath_bet (G.E G) [src] src src"
+    using src_mem_V
+    by (auto intro: dpath_bet_reflexive)
   have "dpath_length [src] = 0"
     by simp
-  also have "... \<le> dist src"
+  also have "... \<le> dist G src src"
     using zero_le
     by (subst zero_enat_def[symmetric])
-  finally have "dpath_length [src] \<le> dist src"
+  finally have "dpath_length [src] \<le> dist G src src"
     .
-  hence "dpath_length [src] = dist src"
-    using dpath_bet
-    by (intro G.G.dist_le_dpath_length antisym)
+  hence "dpath_length [src] = dist G src src"
+    using E_finite dpath_bet
+    by (intro dist_le_dpath_length antisym)
   moreover have "v = src"
     using assms
-    by (simp add: discovered_def dom_def init_def map_empty)
-  moreover have "rev (parent.follow (lookup (parent init)) src) = [src]"
+    by (simp add: discovered_def init_def P.map_empty)
+  moreover have "rev (parent.follow (P_lookup (parent (init src))) src) = [src]"
     using parent_init
     by (simp add: parent_src_init parent.follow_psimps)
   ultimately show ?thesis
@@ -1193,16 +1261,16 @@ qed
 
 subsubsection \<open>@{thm bfs_invar.black_imp_out_neighborhood_not_white}\<close>
 
-lemma (in bfs) black_imp_out_neighborhood_not_white_init:
-  assumes "black init v"
-  shows "\<forall>w\<in>G.set (out_neighborhood v). \<not> white init w"
+lemma (in bfs_invar_tbd) black_imp_out_neighborhood_not_white_init:
+  assumes "black (init src) v"
+  shows "\<forall>w\<in>set (G.out_neighborhood G v). \<not> white (init src) w"
 proof -
   have "v = src"
     using assms
-    by (simp add: discovered_def dom_def init_def map_empty)
-  moreover have "src \<in> set (list (queue init))"
-    using invar_empty
-    by (simp add: init_def list_snoc)
+    by (simp add: discovered_def init_def P.map_empty)
+  moreover have "src \<in> set (Q_list (queue (init src)))"
+    using Q.invar_empty
+    by (simp add: init_def Q.list_snoc)
   ultimately show ?thesis
     using assms
     by blast
@@ -1210,13 +1278,11 @@ qed
 
 subsubsection \<open>\<close>
 
-lemma (in bfs) bfs_invar_init:
-  shows
-    "bfs_invar empty delete isin inorder inv vertices edges out_neighborhood lookup is_empty head tail list insert
-      Map_empty Map_delete Map_invar Queue_empty Queue_invar src update snoc init"
+lemma (in bfs_invar_tbd) bfs_invar_init:
+  shows "bfs_invar'' (init src)"
   using bfs_axioms
   using follow_invar'_parent_init
-  using invar_queue_init queue_distinct_init invar_parent_init parent_src_init
+  using queue_invar_init queue_distinct_init parent_invar_init parent_src_init
   using gray_if_mem_queue_init black_if_mem_ran_init queue_sorted_wrt_dpath_length_init tbd_dpath_length_init
   using not_white_imp_shortest_dpath_init black_imp_out_neighborhood_not_white_init
   by unfold_locales
@@ -1227,40 +1293,40 @@ subsubsection \<open>Convenience Lemmas\<close>
 
 lemma (in bfs_invar) list_queue_non_empty:
   assumes "cond s"
-  shows "list (queue s) \<noteq> []"
-  using invar_queue assms
+  shows "Q_list (queue s) \<noteq> []"
+  using queue_invar assms
   by (intro list_queue_non_empty)
 
 lemma (in bfs_invar) head_queue_imp:
   assumes "cond s"
   shows
-    "head (queue s) \<in> set (list (queue s))"
-    "head (queue s) \<notin> set (list (queue (fold s)))"
+    "Q_head (queue s) \<in> set (Q_list (queue s))"
+    "Q_head (queue s) \<notin> set (Q_list (queue (fold G src s)))"
 proof -
-  let ?u = "head (queue s)"
-  show "?u \<in> set (list (queue s))"
-    using invar_queue assms list_queue_non_empty
-    by (simp add: list_head)
-  hence "?u \<notin> set (filter (Not \<circ> discovered s) (inorder (out_neighborhood (head (queue s)))))"
+  let ?u = "Q_head (queue s)"
+  show "?u \<in> set (Q_list (queue s))"
+    using queue_invar assms list_queue_non_empty
+    by (simp add: Q.list_head)
+  hence "?u \<notin> set (filter (Not \<circ> discovered src s) (G.out_neighborhood G (Q_head (queue s))))"
     using gray_if_mem_queue
     by fastforce
-  moreover have "?u \<notin> set (list (tail (queue s)))"
+  moreover have "?u \<notin> set (Q_list (Q_tail (queue s)))"
     using queue_distinct
-    by (simp add: list_queue[OF invar_queue list_queue_non_empty[OF assms]])
-  ultimately show "?u \<notin> set (list (queue (fold s)))"
+    by (simp add: Q.list_queue[OF queue_invar list_queue_non_empty[OF assms]])
+  ultimately show "?u \<notin> set (Q_list (queue (fold G src s)))"
     using assms
     by (simp add: list_queue_fold_cong)
 qed
 
 lemma (in bfs_invar) head_queue_if:
   assumes "cond s"
-  assumes "v \<in> set (list (queue s))"
-  assumes "v \<notin> set (list (queue (fold s)))"
-  shows "v = head (queue s)"
+  assumes "v \<in> set (Q_list (queue s))"
+  assumes "v \<notin> set (Q_list (queue (fold G src s)))"
+  shows "v = Q_head (queue s)"
 proof -
-  have "list (queue s) = head (queue s) # list (tail (queue s))"
-    using invar_queue assms(1)
-    by (intro list_queue_non_empty list_queue)
+  have "Q_list (queue s) = Q_head (queue s) # Q_list (Q_tail (queue s))"
+    using queue_invar assms(1)
+    by (intro list_queue_non_empty Q.list_queue)
   thus ?thesis
     using assms
     by (simp add: list_queue_fold_cong)
@@ -1268,7 +1334,7 @@ qed
 
 lemma (in bfs_invar) head_queue_iff:
   assumes "cond s"
-  shows "v = head (queue s) \<longleftrightarrow> v \<in> set (list (queue s)) \<and> v \<notin> set (list (queue (fold s)))"
+  shows "v = Q_head (queue s) \<longleftrightarrow> v \<in> set (Q_list (queue s)) \<and> v \<notin> set (Q_list (queue (fold G src s)))"
 proof (standard, goal_cases)
   case 1
   show ?case
@@ -1283,115 +1349,111 @@ next
 qed
 
 lemma (in bfs_invar) not_white_imp_not_white_fold:
-  assumes "cond s"
   assumes "\<not> white s v"
-  shows "\<not> white (fold s) v"
+  shows "\<not> white (fold G src s) v"
   using assms
-  by (auto simp add: discovered_def dom_def lookup_parent_fold_cong)
+  by (auto simp add: discovered_def lookup_parent_fold_cong)
 
 lemma (in bfs_invar) white_not_white_fold_imp:
-  assumes "cond s"
   assumes "white s v"
-  assumes "\<not> white (fold s) v"
+  assumes "\<not> white (fold G src s) v"
   shows
-    "v \<in> G.set (out_neighborhood (head (queue s)))"
-    "lookup (parent (fold s)) v = Some (head (queue s))"
+    "v \<in> set (G.out_neighborhood G (Q_head (queue s)))"
+    "P_lookup (parent (fold G src s)) v = Some (Q_head (queue s))"
 proof -
-  show "v \<in> G.set (out_neighborhood (head (queue s)))"
+  show "v \<in> set (G.out_neighborhood G (Q_head (queue s)))"
     using assms G.out_neighborhood_finite
-    by (fastforce simp add: discovered_def dom_def lookup_parent_fold_cong G.set_def)
-  thus "lookup (parent (fold s)) v = Some (head (queue s))"
+    by (fastforce simp add: discovered_def lookup_parent_fold_cong)
+  thus "P_lookup (parent (fold G src s)) v = Some (Q_head (queue s))"
     using assms G.out_neighborhood_finite
-    by (auto simp add: lookup_parent_fold_cong G.set_def)
+    by (auto simp add: lookup_parent_fold_cong)
 qed
 
 subsubsection \<open>\<close>
 
 lemma (in bfs_invar) follow_invar'_parent_fold:
   assumes "cond s"
-  shows "follow_invar' (lookup (parent (fold s)))"
-  unfolding follow_invar'_def T_fold_cong[OF assms]
+  shows "follow_invar' (P_lookup (parent (fold G src s)))"
+  unfolding follow_invar'_def T_fold_cong
 proof (rule wf_Un)
   let ?r =
-    "{(head (queue s), v) |v.
-      v \<in> set (inorder (out_neighborhood (head (queue s)))) \<and> \<not> discovered s v}"
+    "{(Q_head (queue s), v) |v.
+      v \<in> set (G.out_neighborhood G (Q_head (queue s))) \<and> \<not> discovered src s v}"
   show "wf (T s)"
     using follow_invar'
     by (simp add: follow_invar'_def)
-  have "gray s (head (queue s))"
+  have "gray s (Q_head (queue s))"
     using assms
     by (intro head_queue_imp(1) gray_if_mem_queue) simp+
   thus "wf ?r"
     by (simp add: wf_def)
   show "Domain (T s) \<inter> Range ?r = {}"
     using black_if_mem_ran
-    by (auto simp add: ran_def)
+    by (auto simp add: P.ran_def)
 qed
 
 lemma (in bfs_invar) parent_fold:
   assumes "cond s"
-  shows "Tbd.parent (lookup (parent (fold s)))"
+  shows "Tbd.parent (P_lookup (parent (fold G src s)))"
   using assms
   by unfold_locales (intro follow_invar'_parent_fold)
 
-subsubsection \<open>@{thm bfs_invar.invar_queue}\<close>
+subsubsection \<open>@{thm bfs_invar.queue_invar}\<close>
 
-lemma (in bfs_invar) invar_queue_fold:
+lemma (in bfs_invar) queue_invar_fold:
   assumes "cond s"
-  shows "Queue_invar (queue (fold s))"
-  using invar_queue assms
-  by (intro invar_out_neighborhood invar_queue_fold_2)
+  shows "Q_invar (queue (fold G src s))"
+  using G_invar queue_invar assms
+  by (intro queue_fold_invar_2)
 
 subsubsection \<open>@{thm bfs_invar.queue_distinct}\<close>
 
 lemma (in bfs_invar) queue_distinct_fold:
   assumes "cond s"
-  shows "distinct (list (queue (fold s)))"
+  shows "distinct (Q_list (queue (fold G src s)))"
 proof -
-  let ?l1 = "list (tail (queue s))"
-  let ?l2 = "filter (Not \<circ> discovered s) (inorder (out_neighborhood (head (queue s))))"
-  have list_queue_non_empty: "list (queue s) \<noteq> []"
+  let ?l1 = "Q_list (Q_tail (queue s))"
+  let ?l2 = "filter (Not \<circ> discovered src s) (G.out_neighborhood G (Q_head (queue s)))"
+  have list_queue_non_empty: "Q_list (queue s) \<noteq> []"
     using assms
     by (intro list_queue_non_empty)
   hence "\<And>v. v \<in> set ?l1 \<Longrightarrow> \<not> white s v"
-    using gray_if_mem_queue invar_queue
-    by (auto simp add: list_tail intro: list.set_sel(2))
+    using gray_if_mem_queue queue_invar
+    by (auto simp add: Q.list_tail intro: list.set_sel(2))
   hence "set ?l1 \<inter> set ?l2 = {}"
     by fastforce
   moreover have "distinct ?l1"
-    using queue_distinct invar_queue list_queue_non_empty
-    by (auto simp add: list_tail intro: distinct_tl)
+    using queue_distinct queue_invar list_queue_non_empty
+    by (auto simp add: Q.list_tail intro: distinct_tl)
   moreover have "distinct ?l2"
-    using assms
-    by (intro invar_out_neighborhood G.inorder_distinct distinct_filter)
+    using G_invar
+    by (intro G.out_neighborhood_distinct distinct_filter)
   ultimately show ?thesis
     using assms
     by (simp add: list_queue_fold_cong)
 qed
 
-subsubsection \<open>@{thm bfs_invar.invar_parent}\<close>
+subsubsection \<open>@{thm bfs_invar.parent_invar}\<close>
 
-lemma (in bfs_invar) invar_parent_fold:
-  assumes "cond s"
-  shows "Map_invar (parent (fold s))"
-  using assms invar_parent
-  by (intro invar_out_neighborhood invar_parent_fold_2)
+lemma (in bfs_invar) parent_invar_fold:
+  shows "P_invar (parent (fold G src s))"
+  using G_invar parent_invar
+  by (intro parent_fold_invar_2)
 
 subsubsection \<open>@{thm bfs_invar.parent_src}\<close>
 
 lemma (in bfs_invar) parent_src_fold:
-  assumes "cond s"
-  shows "lookup (parent (fold s)) src = None"
-  using assms invar_parent src_not_white
-  by (simp add: invar_out_neighborhood lookup_parent_fold_cong_2 parent_src)
+  shows "P_lookup (parent (fold G src s)) src = None"
+  using G_invar parent_invar src_not_white
+  by (simp add: lookup_parent_fold_cong_2 parent_src)
 
 subsubsection \<open>@{thm bfs_invar.gray_if_mem_queue}\<close>
 
 lemma (in bfs_invar) gray_if_mem_queue_fold:
   assumes cond: "cond s"
-  assumes mem_queue_fold: "v \<in> set (list (queue (fold s)))"
-  shows "gray (fold s) v"
-proof (cases "v \<in> set (list (queue s))")
+  assumes mem_queue_fold: "v \<in> set (Q_list (queue (fold G src s)))"
+  shows "gray (fold G src s) v"
+proof (cases "v \<in> set (Q_list (queue s))")
   case True
   hence "gray s v"
     by (intro gray_if_mem_queue)
@@ -1400,18 +1462,18 @@ proof (cases "v \<in> set (list (queue s))")
     by blast
 next
   case False
-  have "list (queue s) \<noteq> []"
+  have "Q_list (queue s) \<noteq> []"
     using cond
     by (intro list_queue_non_empty)
-  hence "v \<notin> set (list (tail (queue s)))"
-    using False invar_queue
-    by (auto simp add: list_tail intro: list.set_sel(2))
-  hence "v \<in> set (inorder (out_neighborhood (head (queue s)))) \<and> \<not> discovered s v"
+  hence "v \<notin> set (Q_list (Q_tail (queue s)))"
+    using False queue_invar
+    by (auto simp add: Q.list_tail intro: list.set_sel(2))
+  hence "v \<in> set (G.out_neighborhood G (Q_head (queue s))) \<and> \<not> discovered src s v"
     using mem_queue_fold cond
     by (simp add: list_queue_fold_cong)
-  hence "\<not> white (fold s) v"
+  hence "\<not> white (fold G src s) v"
     using assms(1)
-    by (fastforce simp add: discovered_def dom_def lookup_parent_fold_cong)
+    by (fastforce simp add: discovered_def lookup_parent_fold_cong)
   thus ?thesis
     using mem_queue_fold
     by blast
@@ -1420,38 +1482,36 @@ qed
 subsubsection \<open>@{thm bfs_invar.black_if_mem_ran}\<close>
 
 lemma (in bfs_invar) head_queue_if_2:
-  assumes "cond s"
-  assumes "v \<notin> ran (parent s)"
-  assumes "v \<in> ran (parent (fold s))"
-  shows "v = head (queue s)"
-  using assms invar_out_neighborhood invar_parent
+  assumes "v \<notin> P.ran (parent s)"
+  assumes "v \<in> P.ran (parent (fold G src s))"
+  shows "v = Q_head (queue s)"
+  using assms G_invar parent_invar
   by (auto simp add: ran_parent_fold_cong split: if_splits(2))
 
 lemma (in bfs_invar) black_if_mem_ran_fold:
   assumes cond: "cond s"
-  assumes mem_ran_fold: "v \<in> ran (parent (fold s))"
-  shows "black (fold s) v"
-proof (cases "v \<in> ran (parent s)")
+  assumes mem_ran_fold: "v \<in> P.ran (parent (fold G src s))"
+  shows "black (fold G src s) v"
+proof (cases "v \<in> P.ran (parent s)")
   case True
   show ?thesis
   proof (rule ccontr)
-    assume assm: "\<not> black (fold s) v"
+    assume assm: "\<not> black (fold G src s) v"
     have black: "black s v"
       using True
       by (intro black_if_mem_ran)
-    with cond
-    have not_white_fold: "\<not> white (fold s) v"
+    hence not_white_fold: "\<not> white (fold G src s) v"
       by (intro black_imp_not_white not_white_imp_not_white_fold)
-    have "list (queue s) \<noteq> []"
+    have "Q_list (queue s) \<noteq> []"
       using cond
       by (intro list_queue_non_empty)
-    hence "v \<notin> set (list (tail (queue s)))"
-      using black invar_queue
-      by (auto simp add: list_tail intro: list.set_sel(2))
-    moreover have "v \<in> set (list (queue (fold s)))"
+    hence "v \<notin> set (Q_list (Q_tail (queue s)))"
+      using black queue_invar
+      by (auto simp add: Q.list_tail intro: list.set_sel(2))
+    moreover have "v \<in> set (Q_list (queue (fold G src s)))"
       using assm not_white_fold
       by blast
-    ultimately have "white (fold s) v"
+    ultimately have "white (fold G src s) v"
       using cond black
       by (simp add: discovered_def list_queue_fold_cong)
     thus "False"
@@ -1460,19 +1520,18 @@ proof (cases "v \<in> ran (parent s)")
   qed
 next
   case False
-  have v_eq_head_queue: "v = head (queue s)"
-    using cond invar_queue False mem_ran_fold
+  have v_eq_Q_head_queue: "v = Q_head (queue s)"
+    using queue_invar False mem_ran_fold
     by (intro head_queue_if_2)
-  then have "v \<in> set (list (queue s))"
+  then have "v \<in> set (Q_list (queue s))"
     using cond
     by (blast intro: head_queue_imp(1))
   hence "\<not> white s v"
     by (intro gray_if_mem_queue gray_imp_not_white)
-  with cond
-  have "\<not> white (fold s) v"
+  hence "\<not> white (fold G src s) v"
     by (intro not_white_imp_not_white_fold)
-  moreover have "v \<notin> set (list (queue (fold s)))"
-    unfolding v_eq_head_queue
+  moreover have "v \<notin> set (Q_list (queue (fold G src s)))"
+    unfolding v_eq_Q_head_queue
     using cond
     by (intro head_queue_imp(2))
   ultimately show ?thesis
@@ -1484,7 +1543,7 @@ subsubsection \<open>@{thm bfs_invar.queue_sorted_wrt_dpath_length}\<close>
 lemma (in bfs_invar) not_white_imp_rev_follow_fold_eq_rev_follow:
   assumes "cond s"
   assumes "\<not> white s v"
-  shows "rev (parent.follow (lookup (parent (fold s))) v) = rev (follow v)"
+  shows "rev (parent.follow (P_lookup (parent (fold G src s))) v) = rev (follow v)"
   using assms
 proof (induct v rule: follow.pinduct[OF follow_dom])
   case (1 v)
@@ -1492,13 +1551,13 @@ proof (induct v rule: follow.pinduct[OF follow_dom])
   proof (cases "v = src")
     case True
     hence
-      "lookup (parent s) v = None"
-      "lookup (parent (fold s)) v = None"
-      using parent_src "1.prems"(1) parent_src_fold
+      "P_lookup (parent s) v = None"
+      "P_lookup (parent (fold G src s)) v = None"
+      using parent_src parent_src_fold
       by simp+
     hence
       "rev (follow v) = [v]"
-      "rev (parent.follow (lookup (parent (fold s))) v) = [v]"
+      "rev (parent.follow (P_lookup (parent (fold G src s))) v) = [v]"
       using "1.prems"(1) parent_fold
       by (simp_all add: follow_psimps parent.follow_psimps)
     thus ?thesis
@@ -1506,17 +1565,17 @@ proof (induct v rule: follow.pinduct[OF follow_dom])
   next
     case False
     then obtain u where u:
-      "lookup (parent s) v = Some u"
+      "P_lookup (parent s) v = Some u"
       "\<not> white s u"
       using False "1.prems"(2) black_if_mem_ran
-      by (auto simp add: discovered_def dom_def ran_def)
-    moreover hence "lookup (parent (fold s)) v = Some u"
-      using "1.prems"
+      by (auto simp add: discovered_def P.ran_def)
+    moreover hence "P_lookup (parent (fold G src s)) v = Some u"
+      using "1.prems"(2)
       by (simp add: lookup_parent_fold_cong map_add_Some_iff)
     ultimately have
       "rev (follow v) = rev (follow u) @ [v]"
-      "rev (parent.follow (lookup (parent (fold s))) v) =
-       rev (parent.follow (lookup (parent (fold s))) u) @ [v]"
+      "rev (parent.follow (P_lookup (parent (fold G src s))) v) =
+       rev (parent.follow (P_lookup (parent (fold G src s))) u) @ [v]"
       using "1.prems"(1) parent_fold
       by (simp_all add: follow_psimps parent.follow_psimps)
     thus ?thesis
@@ -1527,72 +1586,72 @@ qed
 
 lemma (in bfs_invar) mem_filter_imp_dpath_length:
   assumes "cond s"
-  assumes "v \<in> set (filter (Not \<circ> discovered s) (inorder (out_neighborhood (head (queue s)))))"
+  assumes "v \<in> set (filter (Not \<circ> discovered src s) (G.out_neighborhood G (Q_head (queue s))))"
   shows
-    "dpath_length (rev (parent.follow (lookup (parent (fold s))) v)) =
-     dpath_length (rev (parent.follow (lookup (parent (fold s))) (head (queue s)))) + 1"
-    "dpath_length (rev (parent.follow (lookup (parent (fold s))) (last (list (queue s))))) \<le>
-     dpath_length (rev (parent.follow (lookup (parent (fold s))) v))"
+    "dpath_length (rev (parent.follow (P_lookup (parent (fold G src s))) v)) =
+     dpath_length (rev (parent.follow (P_lookup (parent (fold G src s))) (Q_head (queue s)))) + 1"
+    "dpath_length (rev (parent.follow (P_lookup (parent (fold G src s))) (last (Q_list (queue s))))) \<le>
+     dpath_length (rev (parent.follow (P_lookup (parent (fold G src s))) v))"
 proof -
-  let ?u = "head (queue s)"
-  have "lookup (parent (fold s)) v = Some ?u"
+  let ?u = "Q_head (queue s)"
+  have "P_lookup (parent (fold G src s)) v = Some ?u"
     using assms
     by (simp add: lookup_parent_fold_cong)
   hence
-    "rev (parent.follow (lookup (parent (fold s))) v) =
-     rev (parent.follow (lookup (parent (fold s))) ?u) @ [v]"
+    "rev (parent.follow (P_lookup (parent (fold G src s))) v) =
+     rev (parent.follow (P_lookup (parent (fold G src s))) ?u) @ [v]"
     using assms(1) parent_fold
     by (simp add: parent.follow_psimps)
   thus dpath_length_eq:
-    "dpath_length (rev (parent.follow (lookup (parent (fold s))) v)) =
-     dpath_length (rev (parent.follow (lookup (parent (fold s))) (head (queue s)))) + 1"
+    "dpath_length (rev (parent.follow (P_lookup (parent (fold G src s))) v)) =
+     dpath_length (rev (parent.follow (P_lookup (parent (fold G src s))) (Q_head (queue s)))) + 1"
     using assms(1) parent_fold parent.follow_non_empty
     by (fastforce simp add: dpath_length_snoc)
 
   have
-    "dpath_length (rev (parent.follow (lookup (parent (fold s))) (last (list (queue s))))) =
-     dpath_length (rev (follow (last (list (queue s)))))"
+    "dpath_length (rev (parent.follow (P_lookup (parent (fold G src s))) (last (Q_list (queue s))))) =
+     dpath_length (rev (follow (last (Q_list (queue s)))))"
     using assms list_queue_non_empty gray_if_mem_queue
     by (simp add: not_white_imp_rev_follow_fold_eq_rev_follow)
   also have "... \<le> dpath_length (rev (follow ?u)) + 1"
     using assms tbd_dpath_length
     by (simp add: cond_def)
-  also have "... = dpath_length (rev (parent.follow (lookup (parent (fold s))) ?u)) + 1"
+  also have "... = dpath_length (rev (parent.follow (P_lookup (parent (fold G src s))) ?u)) + 1"
     using assms head_queue_imp(1) gray_if_mem_queue
     by (simp add: not_white_imp_rev_follow_fold_eq_rev_follow)
-  also have "... = dpath_length (rev (parent.follow (lookup (parent (fold s))) v))"
+  also have "... = dpath_length (rev (parent.follow (P_lookup (parent (fold G src s))) v))"
     unfolding dpath_length_eq
     ..
   finally show
-    "dpath_length (rev (parent.follow (lookup (parent (fold s))) (last (list (queue s))))) \<le>
-     dpath_length (rev (parent.follow (lookup (parent (fold s))) v))"
+    "dpath_length (rev (parent.follow (P_lookup (parent (fold G src s))) (last (Q_list (queue s))))) \<le>
+     dpath_length (rev (parent.follow (P_lookup (parent (fold G src s))) v))"
     .
 qed
 
 lemma (in bfs_invar) queue_sorted_wrt_dpath_length_fold_aux:
   assumes cond: "cond s"
-  assumes u_mem_tail_queue: "u \<in> set (list (tail (queue s)))"
+  assumes u_mem_Q_tail_queue: "u \<in> set (Q_list (Q_tail (queue s)))"
   assumes v_mem_filter:
-    "v \<in> set (filter (Not \<circ> discovered s) (inorder (out_neighborhood (head (queue s)))))"
+    "v \<in> set (filter (Not \<circ> discovered src s) (G.out_neighborhood G (Q_head (queue s))))"
   shows
-    "dpath_length (rev (parent.follow (lookup (parent (fold s))) u)) \<le>
-     dpath_length (rev (parent.follow (lookup (parent (fold s))) v))"
+    "dpath_length (rev (parent.follow (P_lookup (parent (fold G src s))) u)) \<le>
+     dpath_length (rev (parent.follow (P_lookup (parent (fold G src s))) v))"
 proof -
-  have u_mem_queue: "u \<in> set (list (queue s))"
-    using u_mem_tail_queue invar_queue cond list_queue_non_empty
-    by (auto simp add: list_tail intro: list.set_sel(2))
+  have u_mem_queue: "u \<in> set (Q_list (queue s))"
+    using u_mem_Q_tail_queue queue_invar cond list_queue_non_empty
+    by (auto simp add: Q.list_tail intro: list.set_sel(2))
   have
-    "dpath_length (rev (parent.follow (lookup (parent (fold s))) u)) =
+    "dpath_length (rev (parent.follow (P_lookup (parent (fold G src s))) u)) =
      dpath_length (rev (follow u))"
     using cond u_mem_queue gray_if_mem_queue
     by (simp add: not_white_imp_rev_follow_fold_eq_rev_follow)
-  also have "... \<le> dpath_length (rev (follow (last (list (queue s)))))"
+  also have "... \<le> dpath_length (rev (follow (last (Q_list (queue s)))))"
     using u_mem_queue
     by (intro mem_queue_imp_dpath_length_last_queue)
-  also have "... = dpath_length (rev (parent.follow (lookup (parent (fold s))) (last (list (queue s)))))"
+  also have "... = dpath_length (rev (parent.follow (P_lookup (parent (fold G src s))) (last (Q_list (queue s)))))"
     using cond list_queue_non_empty gray_if_mem_queue
     by (simp add: not_white_imp_rev_follow_fold_eq_rev_follow)
-  also have "... \<le> dpath_length (rev (parent.follow (lookup (parent (fold s))) v))"
+  also have "... \<le> dpath_length (rev (parent.follow (P_lookup (parent (fold G src s))) v))"
     using cond v_mem_filter
     by (intro mem_filter_imp_dpath_length(2))
   finally show ?thesis
@@ -1601,30 +1660,31 @@ qed
 
 lemma (in bfs_invar) tbd_dpath_length_fold_aux:
   assumes cond: "cond s"
-  assumes "\<not> is_empty (queue (fold s))"
+  assumes "\<not> Q_is_empty (queue (fold G src s))"
   shows
-    "dpath_length (rev (parent.follow (lookup (parent (fold s))) (last (list (queue (fold s)))))) \<le>
-     dpath_length (rev (parent.follow (lookup (parent (fold s))) (head (queue s)))) + 1"
-proof (cases "filter (Not \<circ> discovered s) (inorder (out_neighborhood (head (queue s)))) = []")
+    "dpath_length (rev (parent.follow (P_lookup (parent (fold G src s))) (last (Q_list (queue (fold G src s)))))) \<le>
+     dpath_length (rev (parent.follow (P_lookup (parent (fold G src s))) (Q_head (queue s)))) + 1"
+proof (cases "filter (Not \<circ> discovered src s) (G.out_neighborhood G (Q_head (queue s))) = []")
   case True
-  hence list_tail_non_empty: "list (tail (queue s)) \<noteq> []"
-    using assms invar_out_neighborhood invar_queue invar_queue_fold_2
-    by (simp add: list_queue_fold_cong is_empty)
-  hence "last (list (queue (fold s))) = last (list (tail (queue s)))"
+  hence list_tail_non_empty: "Q_list (Q_tail (queue s)) \<noteq> []"
+    using assms G_invar queue_invar queue_fold_invar_2
+    by (simp add: list_queue_fold_cong Q.is_empty)
+
+  hence "last (Q_list (queue (fold G src s))) = last (Q_list (Q_tail (queue s)))"
     unfolding list_queue_fold_cong[OF cond] last_appendL[OF True]
     by blast
-  hence "last (list (queue (fold s))) = last (list (queue s))"
+  hence "last (Q_list (queue (fold G src s))) = last (Q_list (queue s))"
     using list_tail_non_empty
-    by (simp add: list_queue[OF invar_queue list_queue_non_empty[OF assms(1)]])
+    by (simp add: Q.list_queue[OF queue_invar list_queue_non_empty[OF assms(1)]])
   hence
-    "dpath_length (rev (parent.follow (lookup (parent (fold s))) (last (list (queue (fold s)))))) =
-     dpath_length (rev (follow (last (list (queue s)))))"
+    "dpath_length (rev (parent.follow (P_lookup (parent (fold G src s))) (last (Q_list (queue (fold G src s)))))) =
+     dpath_length (rev (follow (last (Q_list (queue s)))))"
     using cond list_queue_non_empty gray_if_mem_queue
     by (simp add: not_white_imp_rev_follow_fold_eq_rev_follow)
-  also have "... \<le> dpath_length (rev (follow (head (queue s)))) + 1"
-    using invar_queue cond list_queue_non_empty tbd_dpath_length
-    by (simp add: is_empty)
-  also have "... = dpath_length (rev (parent.follow (lookup (parent (fold s))) (head (queue s)))) + 1"
+  also have "... \<le> dpath_length (rev (follow (Q_head (queue s)))) + 1"
+    using queue_invar cond list_queue_non_empty tbd_dpath_length
+    by (simp add: Q.is_empty)
+  also have "... = dpath_length (rev (parent.follow (P_lookup (parent (fold G src s))) (Q_head (queue s)))) + 1"
     using cond head_queue_imp(1) gray_if_mem_queue
     by (simp add: not_white_imp_rev_follow_fold_eq_rev_follow)
   finally show ?thesis
@@ -1632,8 +1692,8 @@ proof (cases "filter (Not \<circ> discovered s) (inorder (out_neighborhood (head
 next
   case False
   hence
-    "last (list (queue (fold s))) \<in>
-     set (filter (Not \<circ> discovered s) (inorder (out_neighborhood (head (queue s)))))"
+    "last (Q_list (queue (fold G src s))) \<in>
+     set (filter (Not \<circ> discovered src s) (G.out_neighborhood G (Q_head (queue s))))"
     unfolding list_queue_fold_cong[OF cond] last_appendR[OF False]
     by (intro last_in_set)
   with cond
@@ -1643,69 +1703,69 @@ qed
 
 lemma (in bfs_invar) tbd_dpath_length_fold_aux_2:
   assumes cond: "cond s"
-  assumes "\<not> is_empty (queue (fold s))"
+  assumes "\<not> Q_is_empty (queue (fold G src s))"
   shows
-    "dpath_length (rev (parent.follow (lookup (parent (fold s))) (head (queue s)))) \<le>
-     dpath_length (rev (parent.follow (lookup (parent (fold s))) (head (queue (fold s)))))"
-proof (cases "list (tail (queue s)) = []")
+    "dpath_length (rev (parent.follow (P_lookup (parent (fold G src s))) (Q_head (queue s)))) \<le>
+     dpath_length (rev (parent.follow (P_lookup (parent (fold G src s))) (Q_head (queue (fold G src s)))))"
+proof (cases "Q_list (Q_tail (queue s)) = []")
   case True
-  have "head (queue (fold s)) = hd (list (queue (fold s)))"
-    using assms invar_out_neighborhood invar_queue invar_queue_fold_2
-    by (simp add: is_empty list_head)
+  have "Q_head (queue (fold G src s)) = hd (Q_list (queue (fold G src s)))"
+    using assms G_invar queue_invar queue_fold_invar_2
+    by (simp add: Q.is_empty Q.list_head)
   hence
-    "head (queue (fold s)) =
-     hd (filter (Not \<circ> discovered s) (inorder (out_neighborhood (head (queue s)))))"
+    "Q_head (queue (fold G src s)) =
+     hd (filter (Not \<circ> discovered src s) (G.out_neighborhood G (Q_head (queue s))))"
     using cond True
     by (simp add: list_queue_fold_cong)
   moreover have
-    "filter (Not \<circ> discovered s) (inorder (out_neighborhood (head (queue s)))) \<noteq> []"
-    using assms invar_out_neighborhood invar_queue invar_queue_fold_2 True
-    by (simp add: is_empty list_queue_fold_cong)
-  ultimately have head_queue_fold_mem_filter:
-    "head (queue (fold s)) \<in>
-     set (filter (Not \<circ> discovered s) (inorder (out_neighborhood (head (queue s)))))"
+    "filter (Not \<circ> discovered src s) (G.out_neighborhood G (Q_head (queue s))) \<noteq> []"
+    using assms G_invar queue_invar queue_fold_invar_2 True
+    by (simp add: Q.is_empty list_queue_fold_cong)
+  ultimately have Q_head_queue_fold_mem_filter:
+    "Q_head (queue (fold G src s)) \<in>
+     set (filter (Not \<circ> discovered src s) (G.out_neighborhood G (Q_head (queue s))))"
     using list.set_sel(1)
     by metis
 
   have
-    "dpath_length (rev (parent.follow (lookup (parent (fold s))) (head (queue s)))) =
-     dpath_length (rev (follow (head (queue s))))"
+    "dpath_length (rev (parent.follow (P_lookup (parent (fold G src s))) (Q_head (queue s)))) =
+     dpath_length (rev (follow (Q_head (queue s))))"
     using cond head_queue_imp(1) gray_if_mem_queue
     by (simp add: not_white_imp_rev_follow_fold_eq_rev_follow)
-  also have "... \<le> dpath_length (rev (follow (last (list (queue s)))))"
+  also have "... \<le> dpath_length (rev (follow (last (Q_list (queue s)))))"
     using cond
     by (intro head_queue_imp(1) mem_queue_imp_dpath_length_last_queue)
   also have
-    "... = dpath_length (rev (parent.follow (lookup (parent (fold s))) (last (list (queue s)))))"
+    "... = dpath_length (rev (parent.follow (P_lookup (parent (fold G src s))) (last (Q_list (queue s)))))"
     using cond list_queue_non_empty gray_if_mem_queue
     by (simp add: not_white_imp_rev_follow_fold_eq_rev_follow)
-  also have "... \<le> dpath_length (rev (parent.follow (lookup (parent (fold s))) (head (queue (fold s)))))"
-    using cond head_queue_fold_mem_filter
+  also have "... \<le> dpath_length (rev (parent.follow (P_lookup (parent (fold G src s))) (Q_head (queue (fold G src s)))))"
+    using cond Q_head_queue_fold_mem_filter
     by (intro mem_filter_imp_dpath_length(2))
   finally show ?thesis
     .
 next
   case False
-  have "head (queue (fold s)) = hd (list (queue (fold s)))"
-    using assms invar_out_neighborhood invar_queue invar_queue_fold_2
-    by (simp add: is_empty list_head)
-  hence "head (queue (fold s)) = hd (list (tail (queue s)))"
+  have "Q_head (queue (fold G src s)) = hd (Q_list (queue (fold G src s)))"
+    using assms G_invar queue_invar queue_fold_invar_2
+    by (simp add: Q.is_empty Q.list_head)
+  hence "Q_head (queue (fold G src s)) = hd (Q_list (Q_tail (queue s)))"
     using cond False
     by (simp add: list_queue_fold_cong)
-  hence head_queue_fold_mem_list_queue: "head (queue (fold s)) \<in> set (list (queue s))"
-    using False invar_queue cond list_queue_non_empty
-    by (auto simp add: list_tail intro: list.set_sel(2))
+  hence Q_head_queue_fold_mem_list_queue: "Q_head (queue (fold G src s)) \<in> set (Q_list (queue s))"
+    using False queue_invar cond list_queue_non_empty
+    by (auto simp add: Q.list_tail intro: list.set_sel(2))
 
   have
-    "dpath_length (rev (parent.follow (lookup (parent (fold s))) (head (queue s)))) =
-     dpath_length (rev (follow (head (queue s))))"
+    "dpath_length (rev (parent.follow (P_lookup (parent (fold G src s))) (Q_head (queue s)))) =
+     dpath_length (rev (follow (Q_head (queue s))))"
     using cond head_queue_imp(1) gray_if_mem_queue
     by (simp add: not_white_imp_rev_follow_fold_eq_rev_follow)
-  also have "... \<le> dpath_length (rev (follow (head (queue (fold s)))))"
-    using head_queue_fold_mem_list_queue
+  also have "... \<le> dpath_length (rev (follow (Q_head (queue (fold G src s)))))"
+    using Q_head_queue_fold_mem_list_queue
     by (intro mem_queue_imp_dpath_length_head_queue)
-  also have "... = dpath_length (rev (parent.follow (lookup (parent (fold s))) (head (queue (fold s)))))"
-    using cond head_queue_fold_mem_list_queue gray_if_mem_queue
+  also have "... = dpath_length (rev (parent.follow (P_lookup (parent (fold G src s))) (Q_head (queue (fold G src s)))))"
+    using cond Q_head_queue_fold_mem_list_queue gray_if_mem_queue
     by (simp add: not_white_imp_rev_follow_fold_eq_rev_follow)
   finally show ?thesis
     .
@@ -1715,38 +1775,38 @@ lemma (in bfs_invar) queue_sorted_wrt_dpath_length_fold:
   assumes "cond s"
   shows
     "sorted_wrt
-      (\<lambda>u v. dpath_length (rev (parent.follow (lookup (parent (fold s))) u)) \<le>
-             dpath_length (rev (parent.follow (lookup (parent (fold s))) v)))
-      (list (queue (fold s)))"
+      (\<lambda>u v. dpath_length (rev (parent.follow (P_lookup (parent (fold G src s))) u)) \<le>
+             dpath_length (rev (parent.follow (P_lookup (parent (fold G src s))) v)))
+      (Q_list (queue (fold G src s)))"
 proof -
   let ?P =
-    "\<lambda>u v. dpath_length (rev (parent.follow (lookup (parent (fold s))) u)) \<le>
-           dpath_length (rev (parent.follow (lookup (parent (fold s))) v))"
-  have list_queue_non_empty: "list (queue s) \<noteq> []"
+    "\<lambda>u v. dpath_length (rev (parent.follow (P_lookup (parent (fold G src s))) u)) \<le>
+           dpath_length (rev (parent.follow (P_lookup (parent (fold G src s))) v))"
+  have list_queue_non_empty: "Q_list (queue s) \<noteq> []"
     using assms
     by (intro list_queue_non_empty)
   hence
     "sorted_wrt
       (\<lambda>u v. dpath_length (rev (follow u)) \<le> dpath_length (rev (follow v)))
-      (list (queue s))"
-    using invar_queue queue_sorted_wrt_dpath_length
-    by (simp add: is_empty)
-  hence "sorted_wrt ?P (list (queue s))"
-    using assms gray_if_mem_queue sorted_wrt_mono_rel[of "(list (queue s))"]
+      (Q_list (queue s))"
+    using queue_invar queue_sorted_wrt_dpath_length
+    by (simp add: Q.is_empty)
+  hence "sorted_wrt ?P (Q_list (queue s))"
+    using assms gray_if_mem_queue sorted_wrt_mono_rel[of "(Q_list (queue s))"]
     by (simp add: not_white_imp_rev_follow_fold_eq_rev_follow)
-  hence "sorted_wrt ?P (list (tail (queue s)))"
-    by (simp add: list_queue[OF invar_queue list_queue_non_empty])
+  hence "sorted_wrt ?P (Q_list (Q_tail (queue s)))"
+    by (simp add: Q.list_queue[OF queue_invar list_queue_non_empty])
   moreover have
     "sorted_wrt
       ?P
-      (filter (Not \<circ> discovered s) (inorder (out_neighborhood (head (queue s)))))"
+      (filter (Not \<circ> discovered src s) (G.out_neighborhood G (Q_head (queue s))))"
     using assms
     by (auto simp add: mem_filter_imp_dpath_length(1) intro: sorted_wrt_if)
   moreover have
-    "\<forall>u\<in>set (list (tail (queue s))).
-      \<forall>v\<in>set (filter (Not \<circ> discovered s) (inorder (out_neighborhood (head (queue s))))).
-       dpath_length (rev (parent.follow (lookup (parent (fold s))) u)) \<le>
-       dpath_length (rev (parent.follow (lookup (parent (fold s))) v))"
+    "\<forall>u\<in>set (Q_list (Q_tail (queue s))).
+      \<forall>v\<in>set (filter (Not \<circ> discovered src s) (G.out_neighborhood G (Q_head (queue s)))).
+       dpath_length (rev (parent.follow (P_lookup (parent (fold G src s))) u)) \<le>
+       dpath_length (rev (parent.follow (P_lookup (parent (fold G src s))) v))"
     using assms
     by (blast intro: queue_sorted_wrt_dpath_length_fold_aux)
   ultimately show ?thesis 
@@ -1755,18 +1815,18 @@ proof -
 qed
 
 lemma (in bfs_invar) tbd_dpath_length_fold:
-  assumes cond: "cond s"
-  assumes "\<not> is_empty (queue (fold s))"
+  assumes "cond s"
+  assumes "\<not> Q_is_empty (queue (fold G src s))"
   shows
-    "dpath_length (rev (parent.follow (lookup (parent (fold s))) (last (list (queue (fold s)))))) \<le>
-     dpath_length (rev (parent.follow (lookup (parent (fold s))) (head (queue (fold s))))) + 1"
+    "dpath_length (rev (parent.follow (P_lookup (parent (fold G src s))) (last (Q_list (queue (fold G src s)))))) \<le>
+     dpath_length (rev (parent.follow (P_lookup (parent (fold G src s))) (Q_head (queue (fold G src s))))) + 1"
 proof -
   have
-    "dpath_length (rev (parent.follow (lookup (parent (fold s))) (last (list (queue (fold s)))))) \<le>
-     dpath_length (rev (parent.follow (lookup (parent (fold s))) (head (queue s)))) + 1"
+    "dpath_length (rev (parent.follow (P_lookup (parent (fold G src s))) (last (Q_list (queue (fold G src s)))))) \<le>
+     dpath_length (rev (parent.follow (P_lookup (parent (fold G src s))) (Q_head (queue s)))) + 1"
     using assms
     by (intro tbd_dpath_length_fold_aux)
-  also have "... \<le> dpath_length (rev (parent.follow (lookup (parent (fold s))) (head (queue (fold s))))) + 1"
+  also have "... \<le> dpath_length (rev (parent.follow (P_lookup (parent (fold G src s))) (Q_head (queue (fold G src s))))) + 1"
     using assms
     by (auto intro: tbd_dpath_length_fold_aux_2)
   finally show ?thesis
@@ -1777,29 +1837,29 @@ subsubsection \<open>@{thm bfs_invar.not_white_imp_shortest_dpath}\<close>
 
 lemma (in bfs_invar) not_white_imp_shortest_dpath_fold_case_1_subcase_3_aux:
   assumes cond: "cond s"
-  assumes dist_less: "dist v < dist (head (queue s)) + 1"
-  assumes dpath_bet: "dpath_bet edges (l @ [u, u']) src v"
-  assumes dpath_length: "dpath_length (l @ [u, u']) = dist v"
+  assumes dist_less: "dist G src v < dist G src (Q_head (queue s)) + 1"
+  assumes dpath_bet: "dpath_bet (G.E G) (l @ [u, u']) src v"
+  assumes dpath_length: "dpath_length (l @ [u, u']) = dist G src v"
   assumes white: "white s v"
   shows "False"
 proof -
-  let ?u = "head (queue s)"
-  have "dist u + 1 = dist v"
-    using dpath_bet dpath_length
-    by (auto intro: G.G.shortest_dpathE_2)
-  hence "dist u + 1 < dist ?u + 1"
+  let ?u = "Q_head (queue s)"
+  have "dist G src u + 1 = dist G src v"
+    using E_finite dpath_bet dpath_length
+    by (auto intro: shortest_dpathE_2)
+  hence "dist G src u + 1 < dist G src ?u + 1"
     using dist_less
     by simp
-  hence "dist u < dist ?u"
+  hence "dist G src u < dist G src ?u"
     unfolding plus_1_eSuc(2) eSuc_mono
     .
   thus ?thesis
   proof (induct s u rule: vertex_color_induct)
     case white
-    have "dist ?u \<le> dist (last (list (queue s)))"
+    have "dist G src ?u \<le> dist G src (last (Q_list (queue s)))"
       using cond list_queue_non_empty
       by (intro mem_queue_imp_dist_head_queue) simp
-    also have "... \<le> dist u"
+    also have "... \<le> dist G src u"
       using white.hyps cond white_imp_dist_ge
       by (simp add: cond_def)
     finally show ?case
@@ -1807,16 +1867,16 @@ proof -
       by simp
   next
     case gray
-    hence "dist ?u \<le> dist u"
+    hence "dist G src ?u \<le> dist G src u"
       by (intro mem_queue_imp_dist_head_queue) simp
     thus ?case
       using gray.prems
       by simp
   next
     case black
-    hence "v \<in> G.set (out_neighborhood u)"
+    hence "v \<in> set (G.out_neighborhood G u)"
       using dpath_bet
-      by (auto simp add: dpath_bet_def intro: dpath_snoc_edge_2 G.mem_out_neighborhood_if_edge)
+      by (auto simp add: dpath_bet_def G.mem_out_neighborhood_iff_edge intro: dpath_snoc_edge_2)
     hence "\<not> white s v"
       using black.hyps black_imp_out_neighborhood_not_white
       by blast
@@ -1829,20 +1889,20 @@ qed
 lemma (in bfs_invar) not_white_imp_shortest_dpath_fold_case_1_aux:
   assumes cond: "cond s"
   assumes white: "white s v"
-  assumes reachable: "reachable edges src v"
-  assumes v_mem_out_neighborhood: "v \<in> G.set (out_neighborhood (head (queue s)))"
-  shows "dist (head (queue s)) + 1 = dist v"
+  assumes reachable: "reachable (G.E G) src v"
+  assumes v_mem_out_neighborhood: "v \<in> set (G.out_neighborhood G (Q_head (queue s)))"
+  shows "dist G src (Q_head (queue s)) + 1 = dist G src v"
 proof (rule antisym, rule ccontr, goal_cases)
   case 1
-  let ?u = "head (queue s)"
-  assume "\<not> dist ?u + 1 \<le> dist v"
-  hence "dist v < dist ?u + 1"
+  let ?u = "Q_head (queue s)"
+  assume "\<not> dist G src ?u + 1 \<le> dist G src v"
+  hence "dist G src v < dist G src ?u + 1"
     by fastforce
   moreover obtain p where
-    "dpath_bet edges p src v"
-    "dpath_length p = dist v"
-    using reachable
-    by (elim G.G.dist_dpath_betE)
+    "dpath_bet (G.E G) p src v"
+    "dpath_length p = dist G src v"
+    using E_finite reachable
+    by (elim dist_dpath_betE)
   ultimately show ?case
     using white
   proof (induct p arbitrary: v rule: dpath_rev_induct)
@@ -1867,55 +1927,52 @@ proof (rule antisym, rule ccontr, goal_cases)
 next
   case 2
   show ?case
-    using cond invar_out_neighborhood v_mem_out_neighborhood G.G.dist_triangle_inequality_edge
+    using cond head_queue_mem_V v_mem_out_neighborhood E_finite dist_triangle_inequality_edge
     by (simp add: G.mem_out_neighborhood_iff_edge)
 qed
 
 lemma (in bfs_invar) not_white_imp_shortest_dpath_fold:
   assumes cond: "cond s"
-  assumes not_white_fold: "\<not> white (fold s) v"
-  shows
-    "dpath_bet edges (rev (parent.follow (lookup (parent (fold s))) v)) src v \<and>
-     dpath_length (rev (parent.follow (lookup (parent (fold s))) v)) = dist v"
+  assumes not_white_fold: "\<not> white (fold G src s) v"
+  shows "is_shortest_dpath G (rev (parent.follow (P_lookup (parent (fold G src s))) v)) src v"
 proof (cases "white s v", standard)
-  let ?u = "head (queue s)"
+  let ?u = "Q_head (queue s)"
   case True
   hence
-    v_mem_out_neighborhood: "v \<in> G.set (out_neighborhood ?u)" and
-    parent_fold_v_eq_head_queue: "lookup (parent (fold s)) v = Some ?u"
+    v_mem_out_neighborhood: "v \<in> set (G.out_neighborhood G ?u)" and
+    parent_fold_v_eq_head_queue: "P_lookup (parent (fold G src s)) v = Some ?u"
     using assms
     by (auto intro: white_not_white_fold_imp)
-  have head_queue_not_white: "\<not> white s ?u"
+  have Q_head_queue_not_white: "\<not> white s ?u"
     using cond
     by (intro head_queue_imp(1) gray_if_mem_queue gray_imp_not_white)
-  hence rev_follow_head_queue_shortest_dpath:
-    "dpath_bet edges (rev (follow ?u)) src ?u \<and> dpath_length (rev (follow ?u)) = dist ?u"
+  hence rev_follow_head_queue_shortest_dpath: "is_shortest_dpath G (rev (follow ?u)) src ?u"
     by (intro not_white_imp_shortest_dpath)
   have
-    "rev (parent.follow (lookup (parent (fold s))) v) =
-     rev (parent.follow (lookup (parent (fold s))) ?u) @ [v]"
+    "rev (parent.follow (P_lookup (parent (fold G src s))) v) =
+     rev (parent.follow (P_lookup (parent (fold G src s))) ?u) @ [v]"
     using cond parent_fold
     by (simp add: parent.follow_psimps parent_fold_v_eq_head_queue)
-  hence rev_follow_fold_eq: "rev (parent.follow (lookup (parent (fold s))) v) = rev (follow ?u) @ [v]"
-    using cond head_queue_not_white
+  hence rev_follow_fold_eq: "rev (parent.follow (P_lookup (parent (fold G src s))) v) = rev (follow ?u) @ [v]"
+    using cond Q_head_queue_not_white
     by (simp add: not_white_imp_rev_follow_fold_eq_rev_follow)
-  thus "dpath_bet edges (rev (parent.follow (lookup (parent (fold s))) v)) src v"
-    using cond invar_out_neighborhood rev_follow_head_queue_shortest_dpath
+  thus "dpath_bet (G.E G) (rev (parent.follow (P_lookup (parent (fold G src s))) v)) src v"
+    using rev_follow_head_queue_shortest_dpath
     using v_mem_out_neighborhood dpath_bet_transitive
     by (fastforce simp add: G.mem_out_neighborhood_iff_edge edge_iff_dpath_bet)
-  hence "reachable edges src v"
+  hence "reachable (G.E G) src v"
     by (auto simp add: reachable_iff_dpath_bet)
   with cond True
-  have "dist v = dist ?u + 1"
+  have "dist G src v = dist G src ?u + 1"
     using True not_white_fold
     by (intro white_not_white_fold_imp(1) not_white_imp_shortest_dpath_fold_case_1_aux[symmetric])
   also have "... = dpath_length (rev (follow ?u)) + 1"
     unfolding plus_enat_simps(1)[symmetric]
     by (simp add: rev_follow_head_queue_shortest_dpath)
-  also have "... = dpath_length (rev (parent.follow (lookup (parent (fold s))) v))"
+  also have "... = dpath_length (rev (parent.follow (P_lookup (parent (fold G src s))) v))"
     using follow_non_empty
     by (simp add: rev_follow_fold_eq dpath_length_snoc)
-  finally show "dpath_length (rev (parent.follow (lookup (parent (fold s))) v)) = dist v"
+  finally show "dpath_length (rev (parent.follow (P_lookup (parent (fold G src s))) v)) = dist G src v"
     by simp
 next
   case False
@@ -1928,14 +1985,14 @@ subsubsection \<open>@{thm bfs_invar.black_imp_out_neighborhood_not_white}\<clos
 
 lemma (in bfs_invar) black_imp_out_neighborhood_not_white_fold:
   assumes cond: "cond s"
-  assumes black_fold: "black (fold s) v"
-  shows "\<forall>w\<in>G.set (out_neighborhood v). \<not> white (fold s) w"
+  assumes black_fold: "black (fold G src s) v"
+  shows "\<forall>w\<in>set (G.out_neighborhood G v). \<not> white (fold G src s) w"
 proof (induct s v rule: vertex_color_induct)
   case white
-  hence "v \<in> set (inorder (out_neighborhood (head (queue s))))"
-    using assms white_not_white_fold_imp(1)
-    by (simp add: G.set_def)
-  hence "v \<in> set (list (queue (fold s)))"
+  hence "v \<in> set (G.out_neighborhood G (Q_head (queue s)))"
+    using assms
+    by (intro white_not_white_fold_imp(1)) simp+
+  hence "v \<in> set (Q_list (queue (fold G src s)))"
     using white cond
     by (simp add: discovered_def list_queue_fold_cong)
   thus ?case
@@ -1943,18 +2000,17 @@ proof (induct s v rule: vertex_color_induct)
     by blast
 next
   case gray
-  hence "v = head (queue s)"
-    using assms invar_queue
+  hence "v = Q_head (queue s)"
+    using assms queue_invar
     by (intro head_queue_if) simp+
   thus ?case
-    using cond
-    by (auto simp add: G.set_def discovered_def dom_def lookup_parent_fold_cong override_on_def)
+    by (auto simp add: discovered_def lookup_parent_fold_cong override_on_def)
 next
   case black
-  hence "\<forall>w\<in>G.set (out_neighborhood v). \<not> white s w"
+  hence "\<forall>w\<in>set (G.out_neighborhood G v). \<not> white s w"
     by (intro black_imp_out_neighborhood_not_white)
   thus ?case
-    using cond not_white_imp_not_white_fold
+    using not_white_imp_not_white_fold
     by blast
 qed
 
@@ -1962,13 +2018,11 @@ subsubsection \<open>\<close>
 
 lemma (in bfs_invar) bfs_invar_fold:
   assumes "cond s"
-  shows
-    "bfs_invar empty delete isin inorder inv vertices edges out_neighborhood lookup is_empty head tail list insert
-      Map_empty Map_delete Map_invar Queue_empty Queue_invar src update snoc (fold s)"
+  shows "bfs_invar'' (fold G src s)"
   using assms
   using bfs_axioms
   using follow_invar'_parent_fold
-  using invar_queue_fold queue_distinct_fold invar_parent_fold parent_src_fold
+  using queue_invar_fold queue_distinct_fold parent_invar_fold parent_src_fold
   using gray_if_mem_queue_fold black_if_mem_ran_fold queue_sorted_wrt_dpath_length_fold tbd_dpath_length_fold
   using not_white_imp_shortest_dpath_fold black_imp_out_neighborhood_not_white_fold
   by unfold_locales
@@ -1976,97 +2030,86 @@ lemma (in bfs_invar) bfs_invar_fold:
 subsection \<open>@{term bfs.loop}\<close>
 
 lemma (in bfs) loop_psimps:
-  assumes
-    "bfs_invar empty delete isin inorder inv vertices edges out_neighborhood lookup is_empty head tail list insert
-      Map_empty Map_delete Map_invar Queue_empty Queue_invar src update snoc s"
-  shows "loop s = (if cond s then loop (fold s) else s)"
+  assumes "bfs_invar' G src s"
+  shows "loop G src s = (if cond s then loop G src (fold G src s) else s)"
 proof -
-  have "Queue_invar (queue s)"
+  have "G.invar G"
     using assms
-    by (intro bfs_invar.invar_queue)
-  moreover have "Map_invar (parent s)"
+    by (intro bfs_invar.axioms(1) bfs_invar_tbd.G_invar)
+  moreover have "Q_invar (queue s)"
     using assms
-    by (intro bfs_invar.invar_parent)
-  moreover have "set (list (queue s)) \<subseteq> vertices"
+    by (intro bfs_invar.queue_invar)
+  moreover have "P_invar (parent s)"
     using assms
-    by (intro bfs_invar.queue_subset_vertices)
-  moreover have "dom (parent s) \<subseteq> vertices"
+    by (intro bfs_invar.parent_invar)
+  moreover have "set (Q_list (queue s)) \<subseteq> G.V G"
     using assms
-    by (intro bfs_invar.dom_parent_subset_vertices)
+    by (intro bfs_invar.queue_subset_V)
+  moreover have "P.dom (parent s) \<subseteq> G.V G"
+    using assms
+    by (intro bfs_invar.dom_parent_subset_V)
   ultimately show ?thesis
-    using loop_dom loop.psimps
-    by meson
+    by (metis loop_dom loop.psimps)
 qed
 
 lemma (in bfs) bfs_induct:
-  assumes
-    "bfs_invar empty delete isin inorder inv vertices edges out_neighborhood lookup is_empty head tail list insert
-      Map_empty Map_delete Map_invar Queue_empty Queue_invar src update snoc s"
-  assumes "\<And>s. loop_dom s \<Longrightarrow> (cond s \<Longrightarrow> P (fold s)) \<Longrightarrow> P s"
-  shows "P s"
+  assumes "bfs_invar' G src s"
+  assumes "\<And>G src s. loop_dom (G, src, s) \<Longrightarrow> (cond s \<Longrightarrow> P G src (fold G src s)) \<Longrightarrow> P G src s"
+  shows "P G src s"
 proof -
-  have "Queue_invar (queue s)"
+  have "G.invar G"
     using assms(1)
-    by (intro bfs_invar.invar_queue)
-  moreover have "Map_invar (parent s)"
+    by (intro bfs_invar.axioms(1) bfs_invar_tbd.G_invar)
+  moreover have "Q_invar (queue s)"
     using assms(1)
-    by (intro bfs_invar.invar_parent)
-  moreover have "set (list (queue s)) \<subseteq> vertices"
+    by (intro bfs_invar.queue_invar)
+  moreover have "P_invar (parent s)"
+    using assms(1)
+    by (intro bfs_invar.parent_invar)
+  moreover have "set (Q_list (queue s)) \<subseteq> G.V G"
     using assms
-    by (intro bfs_invar.queue_subset_vertices)
-  moreover have "dom (parent s) \<subseteq> vertices"
+    by (intro bfs_invar.queue_subset_V)
+  moreover have "P.dom (parent s) \<subseteq> G.V G"
     using assms(1)
-    by (intro bfs_invar.dom_parent_subset_vertices)
+    by (intro bfs_invar.dom_parent_subset_V)
   ultimately show ?thesis
     using assms(2)
     by (blast intro: loop_dom loop.pinduct)
 qed
 
 lemma (in bfs) bfs_invar_loop:
-  assumes
-    "bfs_invar empty delete isin inorder inv vertices edges out_neighborhood lookup is_empty head tail list insert
-      Map_empty Map_delete Map_invar Queue_empty Queue_invar src update snoc s"
-  shows
-    "bfs_invar empty delete isin inorder inv vertices edges out_neighborhood lookup is_empty head tail list insert
-      Map_empty Map_delete Map_invar Queue_empty Queue_invar src update snoc (loop s)"
+  assumes "bfs_invar' G src s"
+  shows "bfs_invar' G src (loop G src s)"
   using assms
 proof (induct rule: bfs_induct[OF assms])
-  case (1 s)
+  case (1 G src s)
   thus ?case
     by (fastforce simp add: loop_psimps intro: bfs_invar.bfs_invar_fold)
 qed
 
-subsection \<open>@{term bfs.bfs}\<close>
+subsection \<open>@{term bfs}\<close>
 
-lemma (in bfs) bfs_invar_bfs:
-  shows
-    "bfs_invar empty delete isin inorder inv vertices edges out_neighborhood lookup is_empty head tail list insert
-      Map_empty Map_delete Map_invar Queue_empty Queue_invar src update snoc bfs"
+lemma (in bfs_invar_tbd) bfs_invar_bfs:
+  shows "bfs_invar'' (bfs G src)"
   using bfs_invar_init
   by (intro bfs_invar_loop)
 
 section \<open>Correctness\<close>
 
-lemma (in bfs) soundness:
-  assumes
-    "bfs_invar empty delete isin inorder inv vertices edges out_neighborhood lookup is_empty head tail list insert
-      Map_empty Map_delete Map_invar Queue_empty Queue_invar src update snoc s"
-  assumes "discovered (loop s) v"
-  shows
-    "dpath_bet edges (rev (parent.follow (lookup (parent (loop s))) v)) src v \<and>
-     dpath_length (rev (parent.follow (lookup (parent (loop s))) v)) = dist v"
+lemma (in bfs_invar_tbd) soundness:
+  assumes "bfs_invar'' s"
+  assumes "discovered src (loop G src s) v"
+  shows "is_shortest_dpath G (rev (parent.follow (P_lookup (parent (loop G src s))) v)) src v"
   using assms bfs_invar_loop bfs_invar.not_white_imp_shortest_dpath
   by fast
 
-lemma (in bfs) completeness:
-  assumes
-    "bfs_invar empty delete isin inorder inv vertices edges out_neighborhood lookup is_empty head tail list insert
-      Map_empty Map_delete Map_invar Queue_empty Queue_invar src update snoc s"
-  assumes "\<not> discovered (loop s) v"
-  shows "\<not> reachable edges src v"
+lemma (in bfs_invar_tbd) completeness:
+  assumes "bfs_invar'' s"
+  assumes "\<not> discovered src (loop G src s) v"
+  shows "\<not> reachable (G.E G) src v"
   using assms
 proof (induct rule: bfs_induct[OF assms(1)])
-  case (1 s)
+  case (1 G src s)
   show ?case
   proof (cases "cond s")
     case True
@@ -2075,10 +2118,11 @@ proof (induct rule: bfs_induct[OF assms(1)])
       by (intro bfs_invar.bfs_invar_fold "1.hyps"(2)) (simp_all add: loop_psimps)
   next
     case False
-    hence "\<not> discovered s v"
+    hence "\<not> discovered src s v"
       using "1.prems"
       by (simp add: loop_psimps)
-    hence "dist v = \<infinity>"
+    from bfs_invar.white_imp_dist_ge[OF "1.prems"(1) this]
+    have "dist G src v = \<infinity>"
       using "1.prems"(1) False bfs_invar.white_imp_dist_ge
       by (fastforce simp add: cond_def)
     thus ?thesis
@@ -2087,27 +2131,27 @@ proof (induct rule: bfs_induct[OF assms(1)])
   qed
 qed
 
-lemma (in bfs) correctness:
-  assumes
-    "bfs_invar empty delete isin inorder inv vertices edges out_neighborhood lookup is_empty head tail list insert
-      Map_empty Map_delete Map_invar Queue_empty Queue_invar src update snoc s"
-  shows
-    "\<And>v.
-      discovered (loop s) v \<Longrightarrow>
-      dpath_bet edges (rev (parent.follow (lookup (parent (loop s))) v)) src v \<and>
-      dpath_length (rev (parent.follow (lookup (parent (loop s))) v)) = dist v"
-    "\<And>v. \<not> discovered (loop s) v \<Longrightarrow> \<not> reachable edges src v"
+abbreviation (in bfs) is_shortest_dpath_Map :: "'n \<Rightarrow> 'a \<Rightarrow> ('q, 'm) state \<Rightarrow> bool" where
+  "is_shortest_dpath_Map G src s \<equiv>
+   \<forall>v. 
+    discovered src s v \<longrightarrow> is_shortest_dpath G (rev (parent.follow (P_lookup (parent s)) v)) src v \<and>
+    \<not> discovered src s v \<longrightarrow> \<not> reachable (G.E G) src v"
+
+lemma (in bfs_invar_tbd) correctness:
+  assumes "bfs_invar'' s"
+  shows "is_shortest_dpath_Map G src (loop G src s)"
   using assms soundness completeness
   by simp+
 
-lemma (in bfs) bfs_correct:
-  shows
-    "\<And>v.
-      discovered bfs v \<Longrightarrow>
-      dpath_bet edges (rev (parent.follow (lookup (parent bfs)) v)) src v \<and>
-      dpath_length (rev (parent.follow (lookup (parent bfs)) v)) = dist v"
-    "\<And>v. \<not> discovered bfs v \<Longrightarrow> \<not> reachable edges src v"
+theorem (in bfs_invar_tbd) bfs_correct:
+  shows "is_shortest_dpath_Map G src (bfs G src)"
   using bfs_invar_init correctness
   by simp+
+
+corollary (in bfs) bfs_correct:
+  assumes "bfs_invar_tbd' G src"
+  shows "is_shortest_dpath_Map G src (bfs G src)"
+  using assms
+  by (intro bfs_invar_tbd.bfs_correct)
 
 end
