Graph_Theory/Dgraph.thy
@@ -8,13 +8,8 @@ section \<open>Graphs\<close>
 
 type_synonym 'a dgraph = "('a \<times> 'a) set"
 
-locale dgraph =
-  fixes G :: "'a dgraph"
-
-locale finite_dgraph = dgraph G for G +
-  assumes edges_finite: "finite G"
-
-lemma (in finite_dgraph) vertices_finite:
+lemma vertices_finite:
+  assumes "finite G"
   shows "finite (dVs G)"
   unfolding dVs_def
 proof -
@@ -25,7 +20,7 @@ proof -
   finally have "?E = (\<lambda>e. {fst e, snd e}) ` G"
     .
   moreover have "finite ..."
-    using edges_finite
+    using assms
     by simp
   ultimately have "finite ?E"
     by simp
@@ -38,60 +33,19 @@ subsection \<open>Neighborhood\<close>
 definition out_neighborhood :: "'a dgraph \<Rightarrow> 'a \<Rightarrow> 'a set" where
   "out_neighborhood G u \<equiv> {v \<in> dVs G. (u, v) \<in> G}"
 
-lemma (in dgraph) mem_out_neighborhood_iff_edge:
+lemma mem_out_neighborhood_iff_edge:
   shows "v \<in> out_neighborhood G u \<longleftrightarrow> (u, v) \<in> G"
   using dVsI(2)
   by (auto simp add: out_neighborhood_def)
 
-lemma (in dgraph) out_neighborhood_subset_vertices:
+lemma out_neighborhood_subset_vertices:
   shows "out_neighborhood G u \<subseteq> dVs G"
   by (simp add: out_neighborhood_def)
 
-lemma (in finite_dgraph) out_neighborhood_finite:
+lemma out_neighborhood_finite:
+  assumes "finite G"
   shows "finite (out_neighborhood G u)"
-  using out_neighborhood_subset_vertices vertices_finite
-  by (rule finite_subset)
-
-section \<open>\<close>
-
-locale finite_dgraph_tbd =
-  finite_dgraph G +
-  Set_by_Ordered where insert = insert
-  for
-    G :: "'a::linorder dgraph" and
-    insert :: "'a \<Rightarrow> 's \<Rightarrow> 's" +
-  fixes out_neighborhood :: "'a \<Rightarrow> 's"
-  assumes invar_out_neighborhood: "v \<in> dVs G \<Longrightarrow> invar (out_neighborhood v)"
-  assumes isin_out_neighborhood_iff_edge: "invar (out_neighborhood u) \<Longrightarrow> isin (out_neighborhood u) v \<longleftrightarrow> (u, v) \<in> G"
-
-lemma (in finite_dgraph_tbd) mem_out_neighborhood_iff_edge:
-  assumes "invar (out_neighborhood u)"
-  shows "v \<in> set (out_neighborhood u) \<longleftrightarrow> (u, v) \<in> G"
-  using assms isin_out_neighborhood_iff_edge
-  by (simp add: invar_def isin set_def)
-
-lemma (in finite_dgraph_tbd) mem_out_neighborhood_if_edge:
-  assumes "(u, v) \<in> G"
-  shows "v \<in> set (out_neighborhood u)"
-proof -
-  have "u \<in> dVs G"
-    using assms
-    by (intro dVsI(1))
-  hence "invar (out_neighborhood u)"
-    by (intro invar_out_neighborhood)
-  thus ?thesis
-    using assms
-    by (simp add: mem_out_neighborhood_iff_edge)
-qed
-
-lemma (in finite_dgraph_tbd) out_neighborhood_subset_vertices:
-  assumes "invar (out_neighborhood u)"
-  shows "set (out_neighborhood u) \<subseteq> dVs G"
-  using assms
-  by (auto simp add: mem_out_neighborhood_iff_edge intro: dVsI(2))
-
-lemma (in finite_dgraph_tbd) out_neighborhood_finite:
-  shows "finite (set (out_neighborhood u))"
-  by (simp add: set_def)
+  using out_neighborhood_subset_vertices assms finite_subset
+  by (fastforce intro: vertices_finite)
 
 end
