Map_Specs_Tbd.thy
@@ -2,6 +2,8 @@ theory Map_Specs_Tbd
   imports "HOL-Data_Structures.Map_Specs"
 begin
 
+section \<open>@{term Map}\<close>
+
 definition (in Map) dom :: "'m \<Rightarrow> 'a set" where
   "dom m \<equiv> {a. lookup m a \<noteq> None}"
 
@@ -22,5 +24,97 @@ proof -
     using assms
     by simp
 qed
+
+section \<open>@{term Map_by_Ordered}\<close>
+
+lemma map_of_eq_Some_imp_mem:
+  assumes "map_of l a = Some b"
+  shows "(a, b) \<in> set l"
+  using assms
+proof (induction l rule: map_of.induct)
+  case 1
+  thus ?case
+    by simp
+next
+  case (2 c _ ps)
+  thus ?case
+    by (cases "a = c") auto
+qed
+
+(* TODO Move somewhere else. *)
+lemma sorted_imp_distinct:
+  assumes "sorted l"
+  shows "distinct l"
+  using assms
+  by (simp add: strict_sorted_sorted_wrt[symmetric] strict_sorted_iff)
+
+lemma map_of_eq_Some_if_mem:
+  assumes "sorted1 l"
+  assumes "(a, b) \<in> set l"
+  shows "map_of l a = Some b"
+  using assms
+proof (induction l rule: map_of.induct)
+  case 1
+  thus ?case
+    by simp
+next
+  case (2 c d ps)
+  show ?case
+  proof (cases "a = c")
+    case True
+    thus ?thesis
+      using "2.prems" sorted_imp_distinct
+      by force
+  next
+    case False
+    thus ?thesis
+      using "2.prems"
+      by (auto intro: sorted_cons "2.IH")
+  qed
+qed
+
+lemma map_of_eq_Some_iff_mem:
+  assumes "sorted1 l"
+  shows "map_of l a = Some b \<longleftrightarrow> (a, b) \<in> set l"
+  using assms
+  by (auto intro: map_of_eq_Some_imp_mem map_of_eq_Some_if_mem)
+
+lemma (in Map_by_Ordered) mem_inorder_iff_lookup_eq_Some:
+  assumes "invar m"
+  shows "lookup m a = Some b \<longleftrightarrow> (a, b) \<in> set (inorder m)"
+  using assms
+  by (simp add: invar_def inorder_lookup map_of_eq_Some_iff_mem)
+
+lemma (in Map_by_Ordered) dom_inorder_cong:
+  assumes "invar m"
+  shows "dom m = fst ` set (inorder m)"
+proof -
+  { fix a
+    have "a \<in> dom m \<longleftrightarrow> (\<exists>b. lookup m a = Some b)"
+      by (simp add: dom_def)
+    also have "... \<longleftrightarrow> (\<exists>b. (a, b) \<in> set (inorder m))"
+      using assms
+      by (simp add: mem_inorder_iff_lookup_eq_Some)
+    also have "... \<longleftrightarrow> (\<exists>p\<in>set (inorder m). a = fst p)"
+      by force
+    also have "... \<longleftrightarrow> a \<in> fst ` set (inorder m)"
+      by (simp add: image_iff)
+    finally have "a \<in> dom m \<longleftrightarrow> a \<in> fst ` set (inorder m)"
+      . }
+  thus ?thesis
+    by blast
+qed
+
+lemma (in Map_by_Ordered) dom_finite:
+  assumes "invar m"
+  shows "finite (dom m)"
+  using assms
+  by (simp add: dom_inorder_cong)
+
+lemma (in Map_by_Ordered) ran_finite:
+  assumes "invar m"
+  shows "finite (ran m)"
+  using assms
+  by (intro dom_finite dom_finite_imp_ran_finite)
 
 end
